---
title: "Limit Theorems for Sequences"
date: 2018-08-13T11:00:48+08:00
menuTitle: "Analysis"
volumes: ["2"]
layout: "note"
issue: 9

---

<!--more-->

<div class="latex-macros">
  {{< raw >}}
    $\newcommand{\br}{\\}$

    $\newcommand{\R}{\mathbb{R}}$
    $\newcommand{\Q}{\mathbb{Q}}$
    $\newcommand{\Z}{\mathbb{Z}}$
    $\newcommand{\N}{\mathbb{N}}$
    $\newcommand{\C}{\mathbb{C}}$
    $\newcommand{\P}{\mathbb{P}}$
    $\newcommand{\F}{\mathbb{F}}$
    $\newcommand{\L}{\mathcal{L}}$
    $\newcommand{\spa}[1]{\text{span}(#1)}$
    $\newcommand{\dist}[1]{\text{dist}(#1)}$
    $\newcommand{\max}[1]{\text{max}(#1)}$
    $\newcommand{\min}[1]{\text{max}(#1)}$
    $\newcommand{\supr}[1]{\text{sup}(#1)}$
    $\newcommand{\infi}[1]{\text{inf}(#1)}$
    $\newcommand{\set}[1]{\{#1\}}$
    $\newcommand{\emptyset}{\varnothing}$
    $\newcommand{\otherwise}{\text{ otherwise }}$
    $\newcommand{\if}{\text{ if }}$
    $\newcommand{\proj}{\text{proj}}$
    $\newcommand{\union}{\cup}$
    $\newcommand{\intercept}{\cap}$
    $\newcommand{\abs}[1]{\left| #1 \right|}$
    $\newcommand{\norm}[1]{\left\lVert#1\right\rVert}$
    $\newcommand{\pare}[1]{\left(#1\right)}$
    $\newcommand{\t}[1]{\text{ #1 }}$
    $\newcommand{\head}{\text H}$
    $\newcommand{\tail}{\text T}$
    $\newcommand{\d}{\text d}$
    $\newcommand{\limu}[2]{\underset{#1 \to #2}\lim}$
    $\newcommand{\inv}[1]{{#1}^{-1}}$
    $\newcommand{\inner}[2]{\langle #1, #2 \rangle}$
    $\newcommand{\nullity}[1]{\text{nullity}(#1)}$
    $\newcommand{\rank}[1]{\text{rank}(#1)}$
    $\newcommand{\var}[1]{\text{var}(#1)}$
    $\newcommand{\tr}[1]{\text{tr}(#1)}$
    $\newcommand{\oto}{\text{ one-to-one }}$
    $\newcommand{\ot}{\text{ onto }}$
    $\newcommand{\ceil}[1]{\lceil#1\rceil}$
    $\newcommand{\floor}[1]{\lfloor#1\rfloor}$
    $\newcommand{\Re}[1]{\text{Re}(#1)}$
    $\newcommand{\Im}[1]{\text{Im}(#1)}$
    $\newcommand{\dom}[1]{\text{dom}(#1)}$


    $\newcommand{\Vcw}[2]{\begin{pmatrix} #1 \br #2 \end{pmatrix}}$
    $\newcommand{\Vce}[3]{\begin{pmatrix} #1 \br #2 \br #3 \end{pmatrix}}$
    $\newcommand{\Vcr}[4]{\begin{pmatrix} #1 \br #2 \br #3 \br #4 \end{pmatrix}}$
    $\newcommand{\Vct}[5]{\begin{pmatrix} #1 \br #2 \br #3 \br #4 \br #5 \end{pmatrix}}$
    $\newcommand{\Vcy}[6]{\begin{pmatrix} #1 \br #2 \br #3 \br #4 \br #5 \br #6 \end{pmatrix}}$
    $\newcommand{\Vcu}[7]{\begin{pmatrix} #1 \br #2 \br #3 \br #4 \br #5 \br #6 \br #7 \end{pmatrix}}$

    $\newcommand{\vcw}[2]{\begin{matrix} #1 \br #2 \end{matrix}}$
    $\newcommand{\vce}[3]{\begin{matrix} #1 \br #2 \br #3 \end{matrix}}$
    $\newcommand{\vcr}[4]{\begin{matrix} #1 \br #2 \br #3 \br #4 \end{matrix}}$
    $\newcommand{\vct}[5]{\begin{matrix} #1 \br #2 \br #3 \br #4 \br #5 \end{matrix}}$
    $\newcommand{\vcy}[6]{\begin{matrix} #1 \br #2 \br #3 \br #4 \br #5 \br #6 \end{matrix}}$
    $\newcommand{\vcu}[7]{\begin{matrix} #1 \br #2 \br #3 \br #4 \br #5 \br #6 \br #7 \end{matrix}}$

    $\newcommand{\Mqw}[2]{\begin{bmatrix} #1 & #2 \end{bmatrix}}$
    $\newcommand{\Mqe}[3]{\begin{bmatrix} #1 & #2 & #3 \end{bmatrix}}$
    $\newcommand{\Mqr}[4]{\begin{bmatrix} #1 & #2 & #3 & #4 \end{bmatrix}}$
    $\newcommand{\Mqt}[5]{\begin{bmatrix} #1 & #2 & #3 & #4 & #5 \end{bmatrix}}$

    $\newcommand{\Mwq}[2]{\begin{bmatrix} #1 \br #2 \end{bmatrix}}$
    $\newcommand{\Meq}[3]{\begin{bmatrix} #1 \br #2 \br #3 \end{bmatrix}}$
    $\newcommand{\Mrq}[4]{\begin{bmatrix} #1 \br #2 \br #3 \br #4 \end{bmatrix}}$
    $\newcommand{\Mtq}[5]{\begin{bmatrix} #1 \br #2 \br #3 \br #4 \br #5 \end{bmatrix}}$

    $\newcommand{\Mqw}[2]{\begin{bmatrix} #1 & #2 \end{bmatrix}}$
    $\newcommand{\Mwq}[2]{\begin{bmatrix} #1 \br #2 \end{bmatrix}}$
    $\newcommand{\Mww}[4]{\begin{bmatrix} #1 & #2 \br #3 & #4 \end{bmatrix}}$
    $\newcommand{\Mqe}[3]{\begin{bmatrix} #1 & #2 & #3 \end{bmatrix}}$
    $\newcommand{\Meq}[3]{\begin{bmatrix} #1 \br #2 \br #3 \end{bmatrix}}$
    $\newcommand{\Mwe}[6]{\begin{bmatrix} #1 & #2 & #3\br #4 & #5 & #6 \end{bmatrix}}$
    $\newcommand{\Mew}[6]{\begin{bmatrix} #1 & #2 \br #3 & #4 \br #5 & #6 \end{bmatrix}}$
    $\newcommand{\Mee}[9]{\begin{bmatrix} #1 & #2 & #3 \br #4 & #5 & #6 \br #7 & #8 & #9 \end{bmatrix}}$
  {{< /raw >}}
</div>

{{% theorem name="" index="9.1" status="" %}}

Convergent sequences are bounded.

{{% proof index="" method="" %}}

Let $(s\_n) $ be a convergent sequence, and let $s = \lim s\_n$.

Arbitrarily choose an $\epsilon > 0 $. Here we choose $\epsilon = 1 $.

Since $(s\_n) $ is convergent, exists $N \in \N$ so that

$$n > N \implies \abs{ s\_n - s } < 1 $$

$$\begin{align\*}
\abs{(s\_n - s) + s } &\leq \abs{ s\_n - s } + \abs{ s } \br
\abs{ s\_n } &\leq \abs{ s\_n - s } + \abs{ s } \br
\abs{ s\_n } - \abs{ s } &\leq \abs{ s\_n - s } \br
\end{align\*}$$

$\because \abs{ s\_n - s } < 1 $

$$\abs{ s\_n } - \abs{ s } < 1 $$

i.e. For all $n > N $, $\abs{ s\_n }  < 1 + \abs{ s } $.

Define $M = \max{ \set{ \abs{ s } + 1, \abs{ s\_1 }, \abs{ s\_2 }, ..., \abs{ s\_N }}}$.

$M$ is an upper bound of $(s\_n)$.

{{% /proof %}}

{{% /theorem %}}

{{% example name="" %}}

Show that $\frac{ 2n + 1 }{ 3n -1 } \to \frac{ 2 }{ 3 }$.

Fix $\epsilon > 0 $, want to find $ N $ s.t. $n > N \implies \abs{ \frac{ 2n+1 }{ 3n-1 } - \frac{ 2 }{ 3 }} < \epsilon$.

$\begin{align\*}
\abs{ \frac{ 2n+1 }{ 3n-1 } - \frac{ 2 }{ 3 }} &< \epsilon \br
\frac{ 5 }{ 3n-1 } &< \epsilon
\end{align\*}$


$N = \frac{5 + \epsilon}{3 \epsilon}$.

{{% /example %}}

{{% theorem name="" index="" status="" %}}

$s\_n \to s \implies \abs{ s\_n } \to \abs{ s }$.

{{% /theorem %}}

{{% theorem name="the subsequence theorem" index="" status="warning" %}}

Let $\set{ t\_n } $ be a subsequence of $\set{ s\_n } $.

$s\_n \to s $, $t\_n \to s \implies t\_n = s\_{f(n)}$.

where $f(n)$ is an increasing function from $\N $ to $\N$ called the **selection function**.

{{% proof index="" name="" %}}

Consider $\epsilon > 0 $, then $\exists N , \abs{s\_n - s} < \epsilon$.

$n \geq N$, some $f(n)$ is increasing, then $f(n) \geq n$.

$f(1) \geq 1$, assume $f(n) \geq n $.

$f(n + 1) > f(n) \because f$ is increasing.

$\therefore f(n + 1) > n $

$\therefore f(n + 1) \geq n +1 $(because $n$ is an integer)

$\abs{ s\_n - s } < \epsilon, n > N $

$t\_n = s\_{f(n)} $

since f(n) > n, then

$n \geq N \implies f(n) \geq N$

$\therefore \abs{ t\_n - s } = \abs{ s\_{f(n)} - s } < \epsilon $

$\therefore t\_n \to s $ is true $\forall s\_n n \geq N$

{{% /proof %}}

{{% /theorem %}}

{{% example name="" %}}

$s\_n \to s $, then $\set{ s\_n } $ is bounded.

Can know this just like the $inf \set{ \abs{ s\_n }}$ problem

assume false

Then $\set{ s\_n } $ either has no upper bound (-sup \set{ s\_n } = \infty)
or has no lower bound.

Consider $\abs{ S\_n } $ we know $\abs{ s\_n } \to s $

so $\set{ \abs{ s\_n }}$ has no upper bound.

Then for any $M $, there is some $n $ with $\abs{s\_n} > M $

Take a subsequence

$t\_1 $ where $t\_1 = s\_{n\_1} $ where $\abs{ s\_{n\_1}} $
$t\_2 $ where $t\_2 = s\_{n\_2} $ where $\abs{ s\_{n\_2}} > 2$


$\abs{ t\_k } > k $

Then $t\_1, t\_2, t\_3 ... $

is subseq

that does not $\to s $

{{% /example %}}

{{% theorem name="Binomial Theorem" index="" status="" %}}

$$\binom{ n }{ k } = \frac{ n! }{ k! (n - k)! } $$

where $n! = n(n-1) ... 3 \times 2 \times 1 $

{{% /theorem %}}

{{% note name="" %}}

It's obvious that $\binom{ n }{ k }  \in \Q$, how prove that it is also in $\Z $.

$n!$

step 1: choose $k $ from $n$ : $\binom{ n }{ k } $

step 2: order them : $k! $

step 3: order the rest : $(n - k)! $

step 4: Put $k $ first than $n-k $ second

$n! =  \binom{ n }{ k } k! \pare{n-k}! $

Hence, $\frac{ n! }{ k! (n - k)! }$ is an integer, because it is the ways to choose $k $ from $n $.

{{% /note %}}

{{% theorem name="" index="" status="" %}}

$$\binom{ n }{ k } = \binom{ n-1 }{ k } + \binom{ n-1 }{ k -1 } $$

{{% /theorem %}}

{{% definition name="Binomial Theorem" status="" %}}

$$(1 + x)^n = \sum\_{ k=0 }^{ n } \binom{ n }{ k }x^k$$

{{% proof index="" method="" %}}

$$P(n): (1 + x)^n = \binom{ n }{ 0 } + \binom{ n }{ 1 }x + \binom{ n }{ 2 }x^2 + ... + \binom{ n }{ n }x^n$$

**The basis:**

When $n = 0, (1 + x)^0 = \binom{ 0 }{ 0 } = 1$

When $n = 1, (1 + x)^1 = \binom{ 1 }{ 0 } + \binom{ 1 }{ 1 }x = 1 + x$

**The Inductive step:**

$\begin{align\*}
(1 + x)^{n + 1} &= (1+ x)^n (1 + x) \br
&= (1 + x)\pare{\binom{ n }{ 0 } + \binom{ n }{ 1 }x + \binom{ n }{ 2 }x^2 + ... + \binom{ n }{ n }x^n} \br
= \binom{ n }{ 0 } + &\binom{ n }{ 1 }x + \binom{ n }{ 2 }x^2 + ... + \binom{ n }{ n }x^n + \br
&\binom{ n }{ 0 } x + \binom{ n }{ 1 }x^2 + ... + \binom{ n }{ n-1 } x^n + \binom{ n }{ n } x^{n+1} \br
&= \binom{ n+1 }{ 0} + \binom{ n+1 }{ 1 }x  + ... + \binom{ n+1 }{ n }x^n + \binom{ n+1 }{ n+1 } x^{n+1} \br
&= \sum\_{ k=0 }^{ n+1 } \binom{ n + 1 }{ k } x^k
\end{align\*}$

{{% /proof %}}

{{% /definition %}}

{{% definition name="Infinity limits" status="" %}}

For a sequence $(s\_n) $, we write lim $s\_n = + \infty$ provided for each $M > 0 $ there is a number $N $ s.t. $n > N $ implies $s\_n > M $.

Henceforth we will say $(s\_n)$ <u>HAS a limit</u> or <u>the limit exists</u> provided $(s\_n)$ converges or diverges to $+\infty $ or diverges to $-\infty $.

{{% /definition %}}

{{% theorem name="" index="" status="" %}}

$s, t$ are not $ +\infty$ or $-\infty$.

**1.** $s\_n \to s \implies \set{ s\_n } $ is bounded.

**2.** $s\_n \to s  \implies k s\_n \to ks $.

**3.** $s\_n \to s, t\_n \to t \implies s\_n + t\_n \to s + t$.

**4.** $s\_n \to s, t\_n \to t \implies s\_nt\_n \to st$.

**5.** $s\_n \to s, s\_n \neq 0,  s \neq 0 \implies \inv{\pare{s\_n}} \to \inv{ s }$.

**6.** $s\_n \to s, t\_n \to t, s\_n, s \neq 0 \implies \frac{ t\_n }{ s\_n } \to \frac{ t }{ s } $.

**7a.** $If p > 0, \frac{ 1 }{ n^p} \to 0 $.

**7b.** $If \abs{ a } < 1, a^n \to 0$.

**7c.** $\sqrt[ n ]{ n } \to 1$.

**7d.** $If a > 0, \sqrt[ n ]{ a } \to 1 $.

{{% /theorem %}}

{{% theorem name="" index="9.9" status="" %}}

Let $(s\_n)$ and $(t\_n) $ be sequences such that $\lim s\_n = +\infty $ and $\lim t\_n > 0 $  ($\lim t\_n$ can be finite or $+\infty$). Then $\lim s\_n t\_n = +\infty $.

{{% /theorem %}}

{{% theorem name="" index="9.10" status="" %}}

Let $(s\_n)$ be a sequence where $ s\_n > 0, s\_n \in \R $.

$$\lim s\_n = +\infty \iff \lim \frac{ 1 }{ s\_n } = 0 $$

{{% /theorem %}}

