---
title: "Linear Dependence and Linear Independence"
date: 2018-07-03T11:03:48+08:00
volumes: ["1"]
layout: "note"
type: "notes"
issue: 5
weight: 105


---

<p class="hide">
  Linearly Dependent, Linearly Independent.
</p>


<!--more-->

<div class="latex-macros">
  {{< raw >}}
    $\newcommand{\br}{\\}$

    $\newcommand{\R}{\mathbb{R}}$
    $\newcommand{\Q}{\mathbb{Q}}$
    $\newcommand{\Z}{\mathbb{Z}}$
    $\newcommand{\N}{\mathbb{N}}$
    $\newcommand{\C}{\mathbb{C}}$
    $\newcommand{\P}{\mathbb{P}}$
    $\newcommand{\F}{\mathbb{F}}$
    $\newcommand{\L}{\mathcal{L}}$
    $\newcommand{\spa}[1]{\text{span}(#1)}$
    $\newcommand{\set}[1]{\{#1\}}$
    $\newcommand{\emptyset}{\varnothing}$
    $\newcommand{\otherwise}{\text{ otherwise }}$
    $\newcommand{\if}{\text{ if }}$
    $\newcommand{\union}{\cup}$
    $\newcommand{\intercept}{\cap}$
    $\newcommand{\abs}[1]{| #1 |}$
    $\newcommand{\pare}[1]{\left\(#1\right\)}$
    $\newcommand{\t}[1]{\text{ #1 }}$
    $\newcommand{\head}{\text H}$
    $\newcommand{\tail}{\text T}$
    $\newcommand{\inv}[1]{{#1}^{-1}}$
    $\newcommand{\nullity}[1]{\text{nullity}(#1)}$
    $\newcommand{\rank}[1]{\text{rank }#1}$
    $\newcommand{\oto}{\text{ one-to-one }}$
    $\newcommand{\ot}{\text{ onto }}$


    $\newcommand{\Vcw}[2]{\begin{bmatrix} #1 \br #2 \end{bmatrix}}$
    $\newcommand{\Vce}[3]{\begin{bmatrix} #1 \br #2 \br #3 \end{bmatrix}}$
    $\newcommand{\Vcr}[4]{\begin{bmatrix} #1 \br #2 \br #3 \br #4 \end{bmatrix}}$
    $\newcommand{\Vct}[5]{\begin{bmatrix} #1 \br #2 \br #3 \br #4 \br #5 \end{bmatrix}}$
    $\newcommand{\Vcy}[6]{\begin{bmatrix} #1 \br #2 \br #3 \br #4 \br #5 \br #6 \end{bmatrix}}$
    $\newcommand{\Vcu}[7]{\begin{bmatrix} #1 \br #2 \br #3 \br #4 \br #5 \br #6 \br #7 \end{bmatrix}}$

    $\newcommand{\Mqw}[2]{\begin{bmatrix} #1 & #2 \end{bmatrix}}$
    $\newcommand{\Mqe}[3]{\begin{bmatrix} #1 & #2 & #3 \end{bmatrix}}$
    $\newcommand{\Mqr}[4]{\begin{bmatrix} #1 & #2 & #3 & #4 \end{bmatrix}}$
    $\newcommand{\Mqt}[5]{\begin{bmatrix} #1 & #2 & #3 & #4 & #5 \end{bmatrix}}$

    $\newcommand{\Mwq}[2]{\begin{bmatrix} #1 \br #2 \end{bmatrix}}$
    $\newcommand{\Meq}[3]{\begin{bmatrix} #1 \br #2 \br #3 \end{bmatrix}}$
    $\newcommand{\Mrq}[4]{\begin{bmatrix} #1 \br #2 \br #3 \br #4 \end{bmatrix}}$
    $\newcommand{\Mtq}[5]{\begin{bmatrix} #1 \br #2 \br #3 \br #4 \br #5 \end{bmatrix}}$

    $\newcommand{\Mqw}[2]{\begin{bmatrix} #1 & #2 \end{bmatrix}}$
    $\newcommand{\Mwq}[2]{\begin{bmatrix} #1 \br #2 \end{bmatrix}}$
    $\newcommand{\Mww}[4]{\begin{bmatrix} #1 & #2 \br #3 & #4 \end{bmatrix}}$
    $\newcommand{\Mqe}[3]{\begin{bmatrix} #1 & #2 & #3 \end{bmatrix}}$
    $\newcommand{\Meq}[3]{\begin{bmatrix} #1 \br #2 \br #3 \end{bmatrix}}$
    $\newcommand{\Mwe}[6]{\begin{bmatrix} #1 & #2 & #3\br #4 & #5 & #6 \end{bmatrix}}$
    $\newcommand{\Mew}[6]{\begin{bmatrix} #1 & #2 \br #3 & #4 \br #5 & #6 \end{bmatrix}}$
    $\newcommand{\Mee}[9]{\begin{bmatrix} #1 & #2 & #3 \br #4 & #5 & #6 \br #7 & #8 & #9 \end{bmatrix}}$
  {{< /raw >}}
</div>

{{% definition name="linearly dependent" %}}
Let $V$ be a vector space over a field $F$. A subset $S \subseteq V$ is called **linearly dependent** if there <u>exist</u> a finite number of distinct vectors $u\_1, u\_2, ..., u\_n \in S$ and $a\_1, a\_2,..., a\_n \in F$, <u>not all zero</u> such that

$$a\_1v\_1 + a\_2v\_2 + ... + a\_nv\_n = 0$$

{{% /definition %}}

{{% example name="$\R^2$" %}}

Prove that $S= \set{(1,0), (0,1), (2,-3)}$ is linearly dependent.

{{% proof name="" %}}
We just need to find <u>one</u> not all zero coefficient solution.

$-2(1,0) + 3(0,1) +1(2,-3) = (0,0)$

$\therefore S$ is linearly dependent.

{{% /proof %}}

{{% /example %}}

{{% definition name="linearly independent" %}}
Let $V$ be a vector space over $F$, a subset of $S\subseteq V$.

$S$ is called **linearly independent** if it is NOT linearly dependent.

Equivalently, $S$ is called **linearly independent** if for <u>every finite</u> subset of vector $v\_1, v\_2, ..., v\_n \in S$ the only solution of the equation (in $a\_i$) $$a\_1v\_1 + a\_2v\_2 + ... + a\_nv\_n = 0$$
is
$$a\_1=a\_2=...=a\_n=0$$

{{% /definition %}}

{{% note name="" %}}

1\. $V/F, \set{\emptyset}$ is linearly independent.

{{% proof name="by contradiction" %}}

Assume that $\emptyset$ is linear dependent.

$v\_1, v\_2, ..., v\_n \in \emptyset$ and $a\_1,a\_2, ..., a\_n \in F$ such that at least one of the $a\_i$s is non-zero and $a\_1v\_1 + a\_2v\_2 + ... + a\_nv\_n = 0$.

However, since there is no $v \in \emptyset$, there doesn't exist a $a$ that is non-zero.

Therefore, the empty set is linearly independent.

{{% /proof %}}

2\. $V/F, \set{v}\ (v \neq 0)$ is linearly independent.


3\. if $0 \in S, S$ is linearly dependent. (In particular, $\set{0}$ is linearly dependent.)

{{% proof name="by contradiction" %}}
Assume that it is linearly dependent:

$\exists a \in F, a\neq 0.$ s.t. $$av=0$$

$\because a\in F$ and $a\neq 0, \therefore a^{-1} \in F$.

$$a^{-1}(av)= a^{-1}0 \implies v = 0$$

This is a contradiction to $v\neq 0$.

{{% /proof %}}

{{% /note %}}


{{% example name="$\R^2$" %}}
$S=\set{(1,0),(0,1)}$ is linearly independent.

{{% proof name="" %}}
$a(1,0) + b(0,1) = (0,0)$

$\implies (a,b) = (0,0)$

$a= 0, b=0$

$\therefore S$ is linearly independent.
{{% /proof %}}
{{% /example %}}

{{% example name="$\R^2$" %}}
$S=\set{(1,1),(3,-3)}$ is linearly independent.

{{% proof name="" %}}
$a(1,1) + b(2,-3) = (0,0)$

$(a+2b,a-3b) = (0,0)$

$$
\begin{align\*}
a+2b=0 \br
a-3b=0
\end{align*}
$$

$\implies (a,b) = (0,0)$

$a= 0, b=0$

$T$ is linearly independent.
{{% /proof %}}
{{% /example %}}

{{% theorem name="" index="1.6" %}}
$V/F, S\_1, S\_2 \subseteq V$.

If $S\_1$ is linearly dependent and $S\_2\supseteq S\_1$, then $S\_2$ is also linearly dependent.

If $S\_1$ is linearly independent and $S\_2 \subseteq S\_1$, then $S\_2$ is also linearly independent.

{{% /theorem %}}

{{% theorem name="" index="1.7" %}}
$V/F, S \subseteq V, v \in V,$ $S$ is linearly independent.

$S \cup \set{v}$ is linearly dependent
$\iff v \in \spa{S}$.

{{% proof name="" %}}

$\impliedby$

$v\in \spa{S}$.

$\therefore \exists v\_1, v\_2, ..., v\_n \in S$ and $a\_1, a\_2, ..., a\_n \in F$ s.t. $$v=a\_1v\_1 + a\_2v\_2 + ... + a\_nv\_n$$

$a\_1v\_1+a\_2v\_2 + ... a\_nv\_n + (-1)v = 0$

$S\cup \set{v}$ is linearly dependent.

$\implies$

$S \cup \set{v}$ is linearly dependent.

$\therefore$ for $v\_1, v\_2, ..., v\_n, v \in S\cup \set{v}, \exists a\_1, a\_2, ..., a\_n \in F$ s.t.

$$a\_1v\_1+a\_2v\_2 + ... + a\_nv\_n + av = 0$$
at least one of $a\_1, a\_2, ... ,a\_n, a$ is non-zero.

Claim $a \neq 0$.

If $a = 0$, then we have
$a\_1v\_1 + a\_2v\_2 + ... + a\_nv\_n = 0$.

Since $S$ is linearly independent $\set{v\_1, v\_2, ..., v\_n} \subseteq S$ is also linearly independent.

From theorem we get $a\_1=a\_2=a\_3= ... = a\_n = 0= a$

This is a contradiction to the condition $a\_1, a\_2, ..., a\_n, a$ not all zero

$\therefore a \neq 0$

$a\_1v\_1+a\_2v\_2 + ... + a\_nv\_n + av = 0$
$av = -a\_1v\_1 -a\_2v\_2 - ... -a\_nv\_n$
$v = -\frac{a\_1}{a}v\_1 -\frac{a\_2}{a}v\_2 - ... -\frac{a\_n}{a}a\_nv\_n$

$\therefore v \in \spa{S}$.

{{% /proof %}}

{{% /theorem %}}

{{% example name="" %}}
$V=\R, F=\R$

$S=\set{1}$

$x\in V = \R$

$\forall r \in \R, S=\set{r}$ is a generating set.

{{% /example %}}

{{% example name="" %}}
$V=\C, F=\C$

$S = {z} \subset V = \C, z \neq z$

$w \in V = \C$

$w = \frac w z \cdot z$

{{% /example %}}

{{% example name="" %}}
$V=\C, F=\R$

$s = {1, z}, z\neq 0$

$w\in V = \C$

NOTTRUE! $w = \frac w z \cdot z$

{{% /example %}}
