---
title: "Linear Transformation"
date: 2018-07-11T11:03:48+08:00
volumes: ["2"]
layout: "note"
type: "notes"
issue: 1
weight: 201


---

<p class="hide">
Linear Transformation, Identity Transformation, Zero Transformation, Kernel (Null Space), Range (Image), Nullity, Rank, One-to-One, Onto.
</p>

<!--more-->

<div class="latex-macros">
  {{< raw >}}
    $\newcommand{\br}{\\}$

    $\newcommand{\R}{\mathbb{R}}$
    $\newcommand{\Q}{\mathbb{Q}}$
    $\newcommand{\Z}{\mathbb{Z}}$
    $\newcommand{\N}{\mathbb{N}}$
    $\newcommand{\C}{\mathbb{C}}$
    $\newcommand{\P}{\mathbb{P}}$
    $\newcommand{\F}{\mathbb{F}}$
    $\newcommand{\L}{\mathcal{L}}$
    $\newcommand{\spa}[1]{\text{span}(#1)}$
    $\newcommand{\set}[1]{\{#1\}}$
    $\newcommand{\emptyset}{\varnothing}$
    $\newcommand{\otherwise}{\text{ otherwise }}$
    $\newcommand{\if}{\text{ if }}$
    $\newcommand{\union}{\cup}$
    $\newcommand{\intercept}{\cap}$
    $\newcommand{\abs}[1]{| #1 |}$
    $\newcommand{\pare}[1]{\left\(#1\right\)}$
    $\newcommand{\t}[1]{\text{ #1 }}$
    $\newcommand{\head}{\text H}$
    $\newcommand{\tail}{\text T}$
    $\newcommand{\d}{\text d}$
    $\newcommand{\inv}[1]{{#1}^{-1}}$
    $\newcommand{\nullity}[1]{\text{nullity}(#1)}$
    $\newcommand{\rank}[1]{\text{rank }#1}$
    $\newcommand{\nullity}[1]{\text{nullity}(#1)}$
    $\newcommand{\oto}{\text{ one-to-one }}$
    $\newcommand{\ot}{\text{ onto }}$


    $\newcommand{\Vcw}[2]{\begin{bmatrix} #1 \br #2 \end{bmatrix}}$
    $\newcommand{\Vce}[3]{\begin{bmatrix} #1 \br #2 \br #3 \end{bmatrix}}$
    $\newcommand{\Vcr}[4]{\begin{bmatrix} #1 \br #2 \br #3 \br #4 \end{bmatrix}}$
    $\newcommand{\Vct}[5]{\begin{bmatrix} #1 \br #2 \br #3 \br #4 \br #5 \end{bmatrix}}$
    $\newcommand{\Vcy}[6]{\begin{bmatrix} #1 \br #2 \br #3 \br #4 \br #5 \br #6 \end{bmatrix}}$
    $\newcommand{\Vcu}[7]{\begin{bmatrix} #1 \br #2 \br #3 \br #4 \br #5 \br #6 \br #7 \end{bmatrix}}$

    $\newcommand{\Mqw}[2]{\begin{bmatrix} #1 & #2 \end{bmatrix}}$
    $\newcommand{\Mqe}[3]{\begin{bmatrix} #1 & #2 & #3 \end{bmatrix}}$
    $\newcommand{\Mqr}[4]{\begin{bmatrix} #1 & #2 & #3 & #4 \end{bmatrix}}$
    $\newcommand{\Mqt}[5]{\begin{bmatrix} #1 & #2 & #3 & #4 & #5 \end{bmatrix}}$

    $\newcommand{\Mwq}[2]{\begin{bmatrix} #1 \br #2 \end{bmatrix}}$
    $\newcommand{\Meq}[3]{\begin{bmatrix} #1 \br #2 \br #3 \end{bmatrix}}$
    $\newcommand{\Mrq}[4]{\begin{bmatrix} #1 \br #2 \br #3 \br #4 \end{bmatrix}}$
    $\newcommand{\Mtq}[5]{\begin{bmatrix} #1 \br #2 \br #3 \br #4 \br #5 \end{bmatrix}}$

    $\newcommand{\Mqw}[2]{\begin{bmatrix} #1 & #2 \end{bmatrix}}$
    $\newcommand{\Mwq}[2]{\begin{bmatrix} #1 \br #2 \end{bmatrix}}$
    $\newcommand{\Mww}[4]{\begin{bmatrix} #1 & #2 \br #3 & #4 \end{bmatrix}}$
    $\newcommand{\Mqe}[3]{\begin{bmatrix} #1 & #2 & #3 \end{bmatrix}}$
    $\newcommand{\Meq}[3]{\begin{bmatrix} #1 \br #2 \br #3 \end{bmatrix}}$
    $\newcommand{\Mwe}[6]{\begin{bmatrix} #1 & #2 & #3\br #4 & #5 & #6 \end{bmatrix}}$
    $\newcommand{\Mew}[6]{\begin{bmatrix} #1 & #2 \br #3 & #4 \br #5 & #6 \end{bmatrix}}$
    $\newcommand{\Mee}[9]{\begin{bmatrix} #1 & #2 & #3 \br #4 & #5 & #6 \br #7 & #8 & #9 \end{bmatrix}}$
  {{< /raw >}}
</div>

{{% definition name="Linear Transformation" %}}

$V/F, W$ is a vector space over a field $F$.

A **linear transformation** (or **linear map**) $T:V \to W$ is a function which satisfies the following properties:

1. $T(v\_1 + v\_2) = T(v\_1) + (v\_2), \forall v\_1, v\_2 \in V.$
2. $T(cv) = cT(v), \forall v \in V, c \in F.$

{{% /definition %}}

{{% example name="" %}}
$T: \R^3 \to \R^2, T(a\_1, a\_2, a\_3) = (2a\_1-a\_3, a\_2 - a\_1).$

$v\_1 = (a\_1, a\_2, a\_3), v\_2 = (b\_1, b\_2, b\_3).$

$\begin{align\*}
  &T((a\_1, a\_2, a\_3)  + (b\_1, b\_2, b\_3)) \br
  &=T(a\_1 + b\_1, a\_2 + b\_2, a\_3 + b\_3) \br
  &=(2(a\_1 + b\_1) - (a\_3 + b\_3), (a\_2 + b\_2) - (a\_1 + b\_1))
\end{align*}$

$T(c(a\_1, a\_2, a\_3)) = T((ca\_1, ca\_2, ca\_3)) = (c(2a-a\_3), c(a\_2 - a\_1))$

$T((a\_1, a\_2, a\_3)) = (2a\_1-a\_3, a\_2 - a\_1)$

$T((b\_1, b\_2, b\_3)) = (2b\_1-b\_3, b\_2 - b\_1)$

$\begin{align\*}
  &T((a\_1, a\_2, a\_3)) + T((b\_1, b\_2, b\_3)) \br
  &= (2a\_1-a\_3, a\_2 - a\_1) + (2b\_1-b\_3, b\_2 - b\_1) \br
  &= ...
\end{align*}$


{{% /example %}}

{{% example name="reflection about x-axis" %}}

$T: \R^2 \to \R^2, T ((a,b)) = (a, -b)$

{{% /example %}}

{{% example name="Rotation" %}}

$T: \R^2 \to \R^2, T(P)=P'. P=(a,b).$

$T(P) = (a\cos \theta - b \sin \theta, a \sin \theta + b \cos \theta)$

{{% /example %}}

{{% properties name="Basic properties of linear transformation" %}}

1. If $T: V \to W$ a linear transformation,

  - $T(0) = 0$

  - $T(v\_1 - v\_2) = T(v\_1) - T(v\_2)$

2. $T: V \to W$is a linear transportation$\iff T(cv\_1 + v\_2) = c T(v\_1) + T(v\_2), \forall v\_1, v\_2 \in V, \forall c \in F$.

{{% proof index="1" name="" %}}

$T(0) = T(0 + 0) = T(0) + T(0) = T(0) + 0 = T(0) + T(0)$

By cancellation law, $0 = T(0)$.

$T(v\_1 - v\_2) = T(v\_1 + (-v\_2))$.

{{% /proof %}}

{{% /properties %}}

{{% example name="" %}}

$\R^2 \to \R^2$.

$T(x, y) = T(x + y, x-y + 1)$ is not a linear transformation.

$T(x, y) = (x, \abs{y})$ is not a linear transformation.

{{% /example %}}

{{% example name="" %}}

$T: M\_{m \times n}(\R) \to M\_{n \times m} (\R)$.

$T(A) = A^t$ is a linear transformation.

{{% /example %}}

{{% example name="" %}}
$T: \P\_n(x) \to \P\_{n-1}(x)$.

$T(f(x)) = f'(x)$ is a linear transformation.

$\begin{align\*}
T(cf(x) + g(x)) &= (cf(x) + g(x))' \br
&= cf'(x) g'(x) \br
&= cT(f(x)) + T(g(x))
\end{align*}$

{{% /example %}}

{{% example name="" %}}

$T:\R^2 \to \R^3$.

$T(a\_1, a\_2) = (a\_1, a\_2, 0)$

{{% /example %}}

{{% definition name="Identity transformation" %}}

$I: V \to V. I(v) = v, \forall v \in V$.

{{% /definition %}}

{{% definition name="zero transformation" %}}

$T: V \to W. T(x) = 0, \forall x \in V$.

{{% proof index="" name="that zero transformation is linear" %}}
$T(cx + y) = 0$.
$T(cx) + T(y) = 0 + 0 = 0$.
{{% /proof %}}

{{% /definition %}}

{{% definition name="kernel (null space), range (image)" %}}

$T: V \to W$ is a linear transformation.

The **kernel** (or **null space**) of $T$ denoted by $N(T)$, and is defined as:

$$N(T) = \set{v \in V \mid T(v) = 0}$$

The **range** (or **image**) of $T$ is denoted by $R(T)$, and is defined as:

$$R(T)= \set{T(x) \in W \mid x \in V}$$

{{% /definition %}}


{{% theorem name="" index="2.1" %}}

$T: V \to W$ is a linear transformation. <br>
$N(T)$ is a subspace of $V$, and $R(T)$ is a subspace of $W$.

{{% proof index="" name="$N(T) \leq V$" %}}

$x, y \in N(T) \implies T(x) = 0, T(y) = 0$. <br>
$T(x + y) = T(x) + T(y) = 0 + 0 = 0.$ <br>
$\therefore x + y \in N(T)$.

$x \in N(T) \implies T(x) = 0, c \in F$. <br>
$T(cx) = cT(x) = c0 = 0$ <br>
$\therefore cx \in N(T)$.

$N(T) \leq V$.

{{% /proof %}}

{{% proof index="" name="$R(T) \leq W$" %}}

$w\_1, w\_2 \in R(T) \implies \exists x\_1, x\_2 \in V, s.t. T(x\_1) = w\_1, T(x\_2) = w\_2$. <br>
$w\_1 + w\_2 = T(x\_1) + T(x\_2) = T(x\_1 + x\_2)$.
$\therefore (w\_1 + w\_2) \in R(T)$.

$w \in R(T) \implies \exists x \in V s.t. T(x) = w$. <br>
$cw = cT(x) = T(cx)$. <br>
$\therefore cw \in R(T)$.

{{% /proof %}}

{{% /theorem %}}

{{% definition name="Nullity, Rank" %}}

$T:V \to W$ is a linear transformation.

The dimension of the null space $N(T)$ is called the **nullity** of $T$ and is denoted by $\nullity{T}$. i.e.

$$\nullity{T} := \dim{N(T)}$$

The dimension of the image $R(T)$ is called the **rank** of $T$ and is denoted by $\rank{T}$. i.e.

$$\rank{T} := \dim{R(T)}$$

{{% /definition %}}

{{% example name="" %}}

$T: \R^n \to \R^m$. $T(x) = Ax, \forall x \in \R^n$.

$\begin{align\*}
T(cx + y) &= A(cx + y) \br
&= A(cx) + Ay \br
&= cAx + Ay \br
&= cT(x) + T(y)
\end{align*}$

$\rank{A} = \rank{T}$.

{{% /example %}}


{{% theorem name="" index="2.2" %}}

$T:V \to W$ is a linear transformation. <br>
If $\beta = \set{x\_1, x\_2, ..., x\_{n}}$ is a basis of $V$, then

$$R(T) = \spa{T(x\_1), T(x\_2), ... T(x\_n)}$$

{{% /theorem %}}


{{% theorem name="Dimension theorem" index="2.3" %}}

Let $T: V \to W$ be a linear transformation. <br>
If $V$ is a finite-dimensional vector space, then

$$\begin{align\*}
\dim V &= \rank{T} + \nullity{T} \br
&=\dim R(T) + \dim N(T)
\end{align*}$$

{{% proof index="" name="" %}}
Let $\dim N(T) = k, N(T) \leq V$, and $\beta = \set{x\_1, x\_2, ..., x\_{k}}$ be a basis of $N(T)$.

Since $N(T) \leq V, \beta$ can be extended to $\gamma $, a basis of $V$. i.e. $\gamma  = \beta \cup \set{y\_1, y\_2, ..., y\_{n-k}} = \set{x\_1, ..., x\_k, y\_1, ..., y\_{n-k}}$, where $n = \dim V$.

Need to prove $S = \set{T(v\_{k + 1}), T(v\_{k + 2}), ..., T(v\_{n})}$ is a basis for $R(T)$.

<hr>

First we prove that $S $ generates $R(T)$.

Let $w \in R(T)$, then $\exists x \in v$ s.t. $T(x) = w$.

Since $\beta$ is a basis of $V, \exists c\_1, c\_2, ..., c\_{n} \in F$, s.t. $x = \sum c\_ix\_i$.

Then

$$T(x) = T(\sum\_{i=1}^{n} c\_ix\_i) = \sum\_{i=1}^{n} c\_i T(x\_i)$$

Since $\forall i = 1, 2, ..., k, T(v\_i) = 0$,

$$\begin{align\*}
R(T) &= \spa{T(x\_i), ..., T(x\_k), T(y\_1), ... , T(y\_{n-k})} \br
&= \spa{T(y\_1), ..., T(y\_{n-k})}
\end{align*}$$

$\therefore R(T) \subseteq \set{T(y\_1), T(y\_2), ..., T(y\_{ n-k })}$.

<hr>

Next we need to prove this set is linearly independent.

Consider the equation, $a\_1T(y\_1) + ... + a\_{n-k}T(y\_{n-k}) = 0$

$\implies T(a\_1y\_1 + a\_2y\_2 + ... + a\_{n-k} y\_{n-k}) = 0$

$\implies \sum\_{i=1}^{n} a\_iy\_i \in N(T)$

Since $\beta = \set{x\_1, x\_2, ..., x\_{k}}$ is a basis of $N(T)$,

$\exists b\_1, b\_2, ..., b\_{k} \in F$ s.t.

$$\sum\_{i=1}^{n-k} a\_iy\_i = b\_1x\_1 + b\_2x\_2 + ... + b\_{k} x\_{k}$$

$-b\_1x\_1  -b\_2x\_2  ...  -b\_{k} x\_{k}  + a\_1y\_1 + a\_2y\_2 + ... + a\_{n-k} y\_{n-k}= 0$(\*)

Since $\set{x\_1, x\_2, ..., x\_{k}, y\_1, y\_2, ..., y\_{n-k}}$ is a basis of $V$, it is a linearly independent set, in particular, for equation (\*) we get

$$-b\_1 = -b\_2 = -b\_k = a\_1 =a\_2 =...= a\_{n-k} = 0$$

$\therefore \set{T(y\_1), T(y\_2), ..., T(y\_{ n-k })}$ is a linearly independent set.

In particular, it forms a basis of $R(T)$.

$\therefore \rank{T} = \dim R(T) = n-k$

Recall that

$$\begin{align\*}
\nullity{T} = \dim N(T) = k \br
\dim V = n
\end{align*}$$


$\therefore \rank{T} + \nullity{T} = \dim V$

{{% /proof %}}

{{% /theorem %}}

{{% theorem name="" index="2.4" %}}

Let $T: V \to W$ be linear transformation,

$$T \text{is one-to-one} \iff N(T) = \set{0}$$

{{% /theorem %}}

{{% remarks name="" %}}

Null space always contains at least one vector, namely, the null vector $0$.

$$0 \in N(T)$$

{{% /remarks %}}


{{% definition name="one-to-one" %}}

$f: X \to Y$.

$f$ is called a **one-to-one** or **injective** if $\forall x\_1, x\_2 \in X$,

$$x\_1 \neq x\_2 \implies f(x\_1) \neq f(x\_2)$$

Equivalently, $f$ is **one-to-one**, if $\forall x\_1, x\_2 \in X$,

$$f(x\_1)=f(x\_2) \implies x\_1 = x\_2$$

Equivalently, $\forall y \in Y$, there exists <u>exactly one</u> $x \in X$ s.t. $f(x) = y$.

{{% proof index="" name="of equivalency" %}}

Assume that $T$ is one-to-one let $x\in N(T) \implies T(x) = 0 =T(0)$.

Since $T$ is one-to-one, $x = 0$.

=================

Assume that $N(T) = \set{0}$

let $x, y \in V, s.t. T(x) = T(y)$

$\implies T(x) - T(y) =0$

$\implies T(x-y) =0$

$\implies x-y \in N(T) = \set{0}$

$\implies x-y = 0$

$\implies x = y$

{{% /proof %}}

{{% /definition %}}

{{% definition name="onto" status="" %}}

If $f: X \to Y $ is a function with range $X $, that is, if $f(X) = Y $, then $f $ is called **onto**.

Equivalently, $f $ is called **onto** or **surjective** if $\forall y \in Y$, <br>

$$\exists x \in X\text{ s.t. }f(x) = y $$

{{% /definition %}}

{{% theorem name="" index="2.5" %}}
$V$ and $W$ <u>finite-dimensional</u> and $\dim V = \dim W = n$, then the following are all equivalent:

1. $T$ is$\oto$
2. $T$ is$\ot$
3. $\rank{T} = \dim V$
3. $\nullity{T} = 0$

{{% proof index="" name="" %}}
$(1) \implies (2)$

Assume $T$ is$\oto$.

$\implies N(T) = {0}$

$\implies \nullity{T} = \dim N(T) = 0$

Now by the dimension theorem, $\nullity{T} + \rank{T} = \dim V$

$\implies \rank{T} = \dim V$

$\dim R(T) = \dim W$

$\because \dim V = \dim W$

$\therefore R(T) \subseteq W$

We have, $R(T)  = W$

FC. $R(T) = W ,T$ is onto

$(ii) \implies (iii)$

Assume that $T$ is onto,
i.e. $R(T) = W$

i.e. $\rank{T} = \dim W = \dim V$

$(iii) \implies (i)$

Assume that $\rank{T} = \dim V$

$\nullity{T} + \rank{T} = \dim V$

{{% /proof %}}

{{% /theorem %}}

{{% theorem name="" index="2.6" %}}

Let $V$ and $W$ be two vector space over field $F ,\dim V = n $.

Let $\set{x\_1, x\_2, ..., x\_{n}}$ is a basis of $V\_0$, Let $\set{w\_1, w\_2, ..., w\_{n}}$ be a set of <u>any vectors</u> in $W$. Then there exists a <u>unique</u> linear transformation $T: V \to W$ s.t. $T(x\_i) = w\_i, \forall i = 1,2, ..., n$.

{{% proof index="" name="" %}}

Analysis:

$\beta = \set{x\_1, x\_2, ..., x\_{n}} \subseteq V \to W \supseteq \gamma = \set{w\_1, w\_2, ..., w\_{n}}$

Want to define: $T: V \to W,$ s.t. $T(x\_1) = w\_1, T(x\_2) = w\_2, T(x\_3) = w\_3$

T: $\beta \subseteq V \to \gamma \subseteq W$

You want to extend $T$ to $V \to W$

Define a linear transformation $\R^3$ to $\R^2$ whose image is the line $y = x$ in $\R^2$.

$y = x$

$w = \spa{\set{(1, 1)}}$

$T: \R^3 \to \R^2$

$\beta = \set{e\_1, e\_2, e\_{3}}$

Define $T(e\_1) = T(e\_2) = T(e\_3)$


$R(T) = \spa{T(e\_1), T(e\_2), T(e\_3)} = \spa{\set{(1, 1)}}$

$T(a, b, c) = T(a\_1e\_1 + a\_2e\_2 + a\_{3} e\_{3})$

$= aT(e\_1) + bT(e\_2) + cT(e\_3) = (a+b+c)(1,1)$

Since $x \in V$ be an arbitrary vector. We need to know $T(x)=?$.

Since $\set{x\_1, x\_2, ..., x\_{n}}$ is a basis,
_
$\exists$ unique scalars $a\_1, a\_2, ..., a\_{n}$ s.t. $x = \sum\_{i=1}^{n} a\_i x\_i$

We define $T(x)$ as $T(x) := \sum\_{i=1}^{n} a\_i w\_i$(\*)

$T$ is linear transformation.

{{% proof index="" name="" %}}

$x, y \in, c \in F$

$\because \set{x\_1, x\_2, ..., x\_{n}}$ is a basis of $V\exists a\_1, a\_2, ..., a\_{n}$ and $b\_1, b\_2, ..., b\_{n} \in F$, s.t.

$x = \sum\ a\_i x\_i$
$x+y = \sum\ b\_i x\_i$

by definition
$T(x+y) = \sum\_{i=1}^{n}(a\_i + b\_i) w\_i$
$= c \sum\_{i=1}^{n} a\_i w\_i + \sum\_{i=1}^{n} b\_iw\_i$

so $T$ is a linear transformation.

need to choose $T(x\_i) = w\_i \forall i$

$x\_i = 0x\_1 + 0x\_2 + ... + 0 x\_{i-1} + 1x\_i + a\_1x\_i+1 + a\_2x\_i+2 + ... + a\_{n} x\_{n}$.

by definition (\*), $T(x\_i) = 0w\_1 + 0w\_2 + ... + 0 w\_{i-1} + 1w\_i + 0w\_i+1 + 0w\_i+2 + ... + 0 w\_{n}$

{{% remarks name="" %}}

Defining $T$ from basis to entire $V$ is called extending $T$ linearly.

{{% /remarks %}}

{{% /proof %}}

{{% proof index="" name="of uniqueness" %}}

Assume that: there is another linear transformation $U: V \to W$ s.t. $U(n\_i) = w\_i, v\_i = 1,2, ..., n$.

We need to show that $U(x) = T(x) \forall x in V$

since $\set{x\_1, x\_2, ..., x\_{n}}$ is a basis of V,

$\exists c\_1, c\_2, ..., c\_{n} \in F$ s.t. $x = \sum\_{i=1}^{n} c\_ix\_i$

Then $U(x)  = U(\sum\_{i=1}^{n} c\_ix\_i) = \sum\_{i=1}^{n} U(x\_i) = \sum\_{i=1}^{n} c\_iw\_i = T(\sum\_{i=1}^{n} c\_ix\_i) = T(x)$

{{% /proof %}}

{{% /proof %}}

{{% /theorem %}}

{{% corollary name="" index="" %}}

$\dim V = n$

Let $\set{x\_i, ..., x\_N}$ be a basis of $V ,\set{w\_1, w\_2, ..., w\_{n}}$ be any subset in $W$.

If $T: V \to W$ and $U:V \to W$ and two linear transformation s.t.

$T(x\_i) = U(x\_i) = w\_i, \forall i = 1, ..., n$

Then $T(x) = U(x), \forall x \in V$.

i.e. $T$ and $U$ are the same linear transformation.


In other words, if two linear transformation from $V$ to $W$ coincide on a basis of $V$, then they coincide everywhere else.


{{% proof index="" name="" %}}

It follows from the uniqueness of the previous theorem.

{{% /proof %}}

{{% /corollary %}}

Find a linear transformation from $\R^3$ to $\R^2$ s.t. $T(1, 0, 0) = (-1, 5)$ and $T(1,1, 0) = (2,3)$

$\set{(1, 0, 0) , (1,1, 0), (0, 0, 1)}$ is a basis of $\R^3$

Choose $T((0, 0, 1))$ to any vector for example $T((0,0,1)) = (0, 0, 0)$.

$(x, y , z) \in R^3$


$T(x,y,z) = $
$(x,y,z) = (x-y) e\_1 + ye + ze\_3$
$= (x-y)(1, 0, 0) + y (1, 1, 0) + z(0, 0, 1)$
$T(x, y, z) = (x-y)(-1,5) +y(2,3) + 2(0, 0)$
$=(-x + y+2y, 5x -5y + 3y) = (-x+3y, 5x-2y)$

