---
title: "Independence"
date: 2019-01-31T10:24:00+08:00
volumes: ["2"]
layout: "note"
type: "notes"
issue: 7
weight: 27

---

<!--more-->

<div class="latex-macros">
  {{< raw >}}
    $\newcommand{\br}{\\}$
    $\newcommand{\R}{\mathbb{R}}$
    $\newcommand{\Q}{\mathbb{Q}}$
    $\newcommand{\Z}{\mathbb{Z}}$
    $\newcommand{\N}{\mathbb{N}}$
    $\newcommand{\C}{\mathbb{C}}$
    $\newcommand{\P}{\mathbb{P}}$
    $\newcommand{\F}{\mathbb{F}}$
    $\newcommand{\L}{\mathcal{L}}$
    $\newcommand{\spa}[1]{\text{span}(#1)}$
    $\newcommand{\dist}[1]{\text{dist}(#1)}$
    $\newcommand{\max}[1]{\text{max}(#1)}$
    $\newcommand{\min}[1]{\text{min}(#1)}$
    $\newcommand{\supr}[1]{\text{sup}(#1)}$
    $\newcommand{\infi}[1]{\text{inf}(#1)}$
    $\newcommand{\ite}[1]{\text{int}(#1)}$
    $\newcommand{\ext}[1]{\text{ext}(#1)}$
    $\newcommand{\bdry}[1]{\partial #1}$
    $\newcommand{\argmax}[1]{\underset{#1}{\text{argmax }}}$
    $\newcommand{\argmin}[1]{\underset{#1}{\text{argmin }}}$
    $\newcommand{\set}[1]{\left\{#1\right\}}$
    $\newcommand{\emptyset}{\varnothing}$
    $\newcommand{\otherwise}{\text{ otherwise }}$
    $\newcommand{\if}{\text{ if }}$
    $\newcommand{\proj}{\text{proj}}$
    $\newcommand{\union}{\cup}$
    $\newcommand{\intercept}{\cap}$
    $\newcommand{\abs}[1]{\left| #1 \right|}$
    $\newcommand{\norm}[1]{\left\lVert#1\right\rVert}$
    $\newcommand{\pare}[1]{\left(#1\right)}$
    $\newcommand{\brac}[1]{\left[#1\right]}$
    $\newcommand{\t}[1]{\text{ #1 }}$
    $\newcommand{\head}{\text H}$
    $\newcommand{\tail}{\text T}$
    $\newcommand{\d}{\text d}$
    $\newcommand{\limu}[2]{\underset{#1 \to #2}\lim}$
    $\newcommand{\der}[2]{\frac{\d #1}{\d #2}}$
    $\newcommand{\derw}[2]{\frac{\d #1^2}{\d^2 #2}}$
    $\newcommand{\pder}[2]{\frac{\partial #1}{\partial #2}}$
    $\newcommand{\pderw}[2]{\frac{\partial^2 #1}{\partial #2^2}}$
    $\newcommand{\pderws}[3]{\frac{\partial^2 #1}{\partial #2 \partial #3}}$
    $\newcommand{\inv}[1]{{#1}^{-1}}$
    $\newcommand{\inner}[2]{\langle #1, #2 \rangle}$
    $\newcommand{\nullity}[1]{\text{nullity}(#1)}$
    $\newcommand{\rank}[1]{\text{rank }#1}$
    $\newcommand{\nullspace}[1]{\mathcal{N}\pare{#1}}$
    $\newcommand{\range}[1]{\mathcal{R}\pare{#1}}$
    $\newcommand{\var}[1]{\text{var}\pare{#1}}$
    $\newcommand{\cov}[1]{\text{cov}(#1)}$
    $\newcommand{\cov}[2]{\text{cov}\pare{#1, #2}}$
    $\newcommand{\tr}[1]{\text{tr}(#1)}$
    $\newcommand{\oto}{\text{ one-to-one }}$
    $\newcommand{\ot}{\text{ onto }}$
    $\newcommand{\ceil}[1]{\lceil#1\rceil}$
    $\newcommand{\floor}[1]{\lfloor#1\rfloor}$
    $\newcommand{\Re}[1]{\text{Re}(#1)}$
    $\newcommand{\Im}[1]{\text{Im}(#1)}$
    $\newcommand{\dom}[1]{\text{dom}(#1)}$
    $\newcommand{\fnext}[1]{\overset{\sim}{#1}}$
    $\newcommand{\transpose}[1]{{#1}^{\text{T}}}$
    $\newcommand{\b}[1]{\boldsymbol{#1}}$
    $\newcommand{\None}[1]{}$
    $\newcommand{\Vcw}[2]{\begin{bmatrix} #1 \br #2 \end{bmatrix}}$
    $\newcommand{\Vce}[3]{\begin{bmatrix} #1 \br #2 \br #3 \end{bmatrix}}$
    $\newcommand{\Vcr}[4]{\begin{bmatrix} #1 \br #2 \br #3 \br #4 \end{bmatrix}}$
    $\newcommand{\Vct}[5]{\begin{bmatrix} #1 \br #2 \br #3 \br #4 \br #5 \end{bmatrix}}$
    $\newcommand{\Vcy}[6]{\begin{bmatrix} #1 \br #2 \br #3 \br #4 \br #5 \br #6 \end{bmatrix}}$
    $\newcommand{\Vcu}[7]{\begin{bmatrix} #1 \br #2 \br #3 \br #4 \br #5 \br #6 \br #7 \end{bmatrix}}$
    $\newcommand{\vcw}[2]{\begin{matrix} #1 \br #2 \end{matrix}}$
    $\newcommand{\vce}[3]{\begin{matrix} #1 \br #2 \br #3 \end{matrix}}$
    $\newcommand{\vcr}[4]{\begin{matrix} #1 \br #2 \br #3 \br #4 \end{matrix}}$
    $\newcommand{\vct}[5]{\begin{matrix} #1 \br #2 \br #3 \br #4 \br #5 \end{matrix}}$
    $\newcommand{\vcy}[6]{\begin{matrix} #1 \br #2 \br #3 \br #4 \br #5 \br #6 \end{matrix}}$
    $\newcommand{\vcu}[7]{\begin{matrix} #1 \br #2 \br #3 \br #4 \br #5 \br #6 \br #7 \end{matrix}}$
    $\newcommand{\Mqw}[2]{\begin{bmatrix} #1 & #2 \end{bmatrix}}$
    $\newcommand{\Mqe}[3]{\begin{bmatrix} #1 & #2 & #3 \end{bmatrix}}$
    $\newcommand{\Mqr}[4]{\begin{bmatrix} #1 & #2 & #3 & #4 \end{bmatrix}}$
    $\newcommand{\Mqt}[5]{\begin{bmatrix} #1 & #2 & #3 & #4 & #5 \end{bmatrix}}$
    $\newcommand{\Mwq}[2]{\begin{bmatrix} #1 \br #2 \end{bmatrix}}$
    $\newcommand{\Meq}[3]{\begin{bmatrix} #1 \br #2 \br #3 \end{bmatrix}}$
    $\newcommand{\Mrq}[4]{\begin{bmatrix} #1 \br #2 \br #3 \br #4 \end{bmatrix}}$
    $\newcommand{\Mtq}[5]{\begin{bmatrix} #1 \br #2 \br #3 \br #4 \br #5 \end{bmatrix}}$
    $\newcommand{\Mqw}[2]{\begin{bmatrix} #1 & #2 \end{bmatrix}}$
    $\newcommand{\Mwq}[2]{\begin{bmatrix} #1 \br #2 \end{bmatrix}}$
    $\newcommand{\Mww}[4]{\begin{bmatrix} #1 & #2 \br #3 & #4 \end{bmatrix}}$
    $\newcommand{\Mqe}[3]{\begin{bmatrix} #1 & #2 & #3 \end{bmatrix}}$
    $\newcommand{\Meq}[3]{\begin{bmatrix} #1 \br #2 \br #3 \end{bmatrix}}$
    $\newcommand{\Mwe}[6]{\begin{bmatrix} #1 & #2 & #3\br #4 & #5 & #6 \end{bmatrix}}$
    $\newcommand{\Mew}[6]{\begin{bmatrix} #1 & #2 \br #3 & #4 \br #5 & #6 \end{bmatrix}}$
    $\newcommand{\Mee}[9]{\begin{bmatrix} #1 & #2 & #3 \br #4 & #5 & #6 \br #7 & #8 & #9 \end{bmatrix}}$
  {{< /raw >}}
</div>

{{% definition name="Independence between random variable and event" status="" %}}

We say that random variable $X$ is **independent of the event** $A$ if

$$\b{P}({X = x} \cap A) = \b{P}(X = x)\b{P}(A) = p\_X(x)\b{P}(A), \forall x $$

It follows that if $\b{P}(A) \neq 0$, independence is the same as the condition

$$p\_{X|A} (x) = p\_X(x), \forall x $$

{{% /definition %}}

{{% definition name="Independence of Random Variables" status="" %}}

We say that two **random variables** $X$ and $Y$ are **independent** if

$$p\_{X,Y}(x, y) = p\_X(x)p\_Y(y), \forall x, y$$

It follows that

$$p\_{X|Y}(x|y) = p\_X(x), \forall y, p\_Y(y) \neq 0, \forall x$$

$$p\_{Y|X}(y|) = p\_Y(y), \forall x, p\_X(x) \neq 0, \forall y$$

{{% /definition %}}

{{% definition name="Conditional independence" status="" %}}

Given an event $A$, $\b{P}(A) \neq 0$, we say random variables $X$ and $Y$ are **conditionally independent** if

$$\b{P}(X=x,Y=y|A)=\b{P}(X=x|A)\b{P}(Y=y|A), \forall x,y$$

or in another notation,

$p\_{X,Y|A}(x, y) = p\_{X|A}(x)p\_{Y|A}(y), \forall x, y$

Once more, this is equivalent to

$p\_{X|Y, A} (x|y) = p\_{X|A}(x) \forall x, y, p\_{Y|A}(y) > 0$

{{% /definition %}}

{{% theorem name="Expectation of the product of two random variables" index="" status="" %}}

If $X$ and $Y$ are independent random variables, then

$$E\brac{ XY } = E\brac{ X } E\brac{ Y } $$

as shown by the following calculation,

$$\begin{align}
E\brac{ XY } &= \sum\_{ x } \sum\_{ y }xy p\_{X,Y}(x, y) \br
&= \sum\_{ x } \sum\_{ x }xy p\_X(x) p\_Y(y) \br
&= \sum\_{ x } x p\_X(x) \sum\_{ y } y p\_Y(y) \br
&= E\brac{ X } E\brac{ Y }
\end{align}$$

Similarly,

$$E\brac{ g(X) h(Y)} = E\brac{ g(X)} E\brac{ h(Y)} $$

{{% /theorem %}}

{{% theorem name="Variance of the sum of two independent random variables" index="" status="" %}}

Let $X$ and $Y$ be two independent random variables. Let $\tilde X = X - E\brac{ X } $ and $\tilde Y = Y - E\brac{ Y } $. We have

$$\begin{align\*}
\var{ X+Y } &= \var{ \tilde X + \tilde Y } \br
&= E\brac{(\tilde X + \tilde Y)^2 } \br
&= E\brac{{\tilde X}^2 + 2 \tilde X \tilde Y + {\tilde Y}^2 } \br
&= E\brac{{\tilde X}^2 } + 2 E\brac{ \tilde X \tilde Y } + E\brac{{\tilde Y}^2 } \br
&= E\brac{{\tilde X}^2 }  + E\brac{{\tilde Y}^2 } \br
&= \var{ \tilde X } + \var{ \tilde Y } \br
&= \var{ X } + \var{ Y }
\end{align\*}$$

In conclusion, the variance of the sum of two **independent** random variables is equal to the sum of their variances.

{{% /theorem %}}

