---
title: "Transforms"
date: 2019-01-31T13:30:00+08:00
volumes: ["4"]
layout: "note"
issue: 4
weight: 44

---

<!--more-->

<div class="latex-macros">
  {{< raw >}}
    $\newcommand{\br}{\\}$
    $\newcommand{\R}{\mathbb{R}}$
    $\newcommand{\Q}{\mathbb{Q}}$
    $\newcommand{\Z}{\mathbb{Z}}$
    $\newcommand{\N}{\mathbb{N}}$
    $\newcommand{\C}{\mathbb{C}}$
    $\newcommand{\P}{\mathbb{P}}$
    $\newcommand{\F}{\mathbb{F}}$
    $\newcommand{\L}{\mathcal{L}}$
    $\newcommand{\spa}[1]{\text{span}(#1)}$
    $\newcommand{\dist}[1]{\text{dist}(#1)}$
    $\newcommand{\max}[1]{\text{max}(#1)}$
    $\newcommand{\min}[1]{\text{max}(#1)}$
    $\newcommand{\supr}[1]{\text{sup}(#1)}$
    $\newcommand{\infi}[1]{\text{inf}(#1)}$
    $\newcommand{\ite}[1]{\text{int}(#1)}$
    $\newcommand{\ext}[1]{\text{ext}(#1)}$
    $\newcommand{\bdry}[1]{\partial #1}$
    $\newcommand{\argmax}[1]{\underset{#1}{\text{argmax }}}$
    $\newcommand{\argmin}[1]{\underset{#1}{\text{argmin }}}$
    $\newcommand{\set}[1]{\left\{#1\right\}}$
    $\newcommand{\emptyset}{\varnothing}$
    $\newcommand{\tilde}{\text{~}}$
    $\newcommand{\otherwise}{\text{ otherwise }}$
    $\newcommand{\if}{\text{ if }}$
    $\newcommand{\proj}{\text{proj}}$
    $\newcommand{\union}{\cup}$
    $\newcommand{\intercept}{\cap}$
    $\newcommand{\abs}[1]{\left| #1 \right|}$
    $\newcommand{\norm}[1]{\left\lVert#1\right\rVert}$
    $\newcommand{\pare}[1]{\left(#1\right)}$
    $\newcommand{\brac}[1]{\left[#1\right]}$
    $\newcommand{\t}[1]{\text{ #1 }}$
    $\newcommand{\head}{\text H}$
    $\newcommand{\tail}{\text T}$
    $\newcommand{\d}{\text d}$
    $\newcommand{\limu}[2]{\underset{#1 \to #2}\lim}$
    $\newcommand{\der}[2]{\frac{\d #1}{\d #2}}$
    $\newcommand{\derw}[2]{\frac{\d #1^2}{\d^2 #2}}$
    $\newcommand{\pder}[2]{\frac{\partial #1}{\partial #2}}$
    $\newcommand{\pderw}[2]{\frac{\partial^2 #1}{\partial #2^2}}$
    $\newcommand{\pderws}[3]{\frac{\partial^2 #1}{\partial #2 \partial #3}}$
    $\newcommand{\inv}[1]{{#1}^{-1}}$
    $\newcommand{\inner}[2]{\langle #1, #2 \rangle}$
    $\newcommand{\nullity}[1]{\text{nullity}(#1)}$
    $\newcommand{\rank}[1]{\text{rank }#1}$
    $\newcommand{\nullspace}[1]{\mathcal{N}\pare{#1}}$
    $\newcommand{\range}[1]{\mathcal{R}\pare{#1}}$
    $\newcommand{\var}[1]{\text{var}\pare{#1}}$
    $\newcommand{\cov}[1]{\text{cov}(#1)}$
    $\newcommand{\cov}[2]{\text{cov}\pare{#1, #2}}$
    $\newcommand{\tr}[1]{\text{tr}(#1)}$
    $\newcommand{\oto}{\text{ one-to-one }}$
    $\newcommand{\ot}{\text{ onto }}$
    $\newcommand{\ceil}[1]{\lceil#1\rceil}$
    $\newcommand{\floor}[1]{\lfloor#1\rfloor}$
    $\newcommand{\Re}[1]{\text{Re}(#1)}$
    $\newcommand{\Im}[1]{\text{Im}(#1)}$
    $\newcommand{\dom}[1]{\text{dom}(#1)}$
    $\newcommand{\fnext}[1]{\overset{\sim}{#1}}$
    $\newcommand{\transpose}[1]{{#1}^{\text{T}}}$
    $\newcommand{\b}[1]{\boldsymbol{#1}}$
    $\newcommand{\None}[1]{}$
    $\newcommand{\Vcw}[2]{\begin{bmatrix} #1 \br #2 \end{bmatrix}}$
    $\newcommand{\Vce}[3]{\begin{bmatrix} #1 \br #2 \br #3 \end{bmatrix}}$
    $\newcommand{\Vcr}[4]{\begin{bmatrix} #1 \br #2 \br #3 \br #4 \end{bmatrix}}$
    $\newcommand{\Vct}[5]{\begin{bmatrix} #1 \br #2 \br #3 \br #4 \br #5 \end{bmatrix}}$
    $\newcommand{\Vcy}[6]{\begin{bmatrix} #1 \br #2 \br #3 \br #4 \br #5 \br #6 \end{bmatrix}}$
    $\newcommand{\Vcu}[7]{\begin{bmatrix} #1 \br #2 \br #3 \br #4 \br #5 \br #6 \br #7 \end{bmatrix}}$
    $\newcommand{\vcw}[2]{\begin{matrix} #1 \br #2 \end{matrix}}$
    $\newcommand{\vce}[3]{\begin{matrix} #1 \br #2 \br #3 \end{matrix}}$
    $\newcommand{\vcr}[4]{\begin{matrix} #1 \br #2 \br #3 \br #4 \end{matrix}}$
    $\newcommand{\vct}[5]{\begin{matrix} #1 \br #2 \br #3 \br #4 \br #5 \end{matrix}}$
    $\newcommand{\vcy}[6]{\begin{matrix} #1 \br #2 \br #3 \br #4 \br #5 \br #6 \end{matrix}}$
    $\newcommand{\vcu}[7]{\begin{matrix} #1 \br #2 \br #3 \br #4 \br #5 \br #6 \br #7 \end{matrix}}$
    $\newcommand{\Mqw}[2]{\begin{bmatrix} #1 & #2 \end{bmatrix}}$
    $\newcommand{\Mqe}[3]{\begin{bmatrix} #1 & #2 & #3 \end{bmatrix}}$
    $\newcommand{\Mqr}[4]{\begin{bmatrix} #1 & #2 & #3 & #4 \end{bmatrix}}$
    $\newcommand{\Mqt}[5]{\begin{bmatrix} #1 & #2 & #3 & #4 & #5 \end{bmatrix}}$
    $\newcommand{\Mwq}[2]{\begin{bmatrix} #1 \br #2 \end{bmatrix}}$
    $\newcommand{\Meq}[3]{\begin{bmatrix} #1 \br #2 \br #3 \end{bmatrix}}$
    $\newcommand{\Mrq}[4]{\begin{bmatrix} #1 \br #2 \br #3 \br #4 \end{bmatrix}}$
    $\newcommand{\Mtq}[5]{\begin{bmatrix} #1 \br #2 \br #3 \br #4 \br #5 \end{bmatrix}}$
    $\newcommand{\Mqw}[2]{\begin{bmatrix} #1 & #2 \end{bmatrix}}$
    $\newcommand{\Mwq}[2]{\begin{bmatrix} #1 \br #2 \end{bmatrix}}$
    $\newcommand{\Mww}[4]{\begin{bmatrix} #1 & #2 \br #3 & #4 \end{bmatrix}}$
    $\newcommand{\Mqe}[3]{\begin{bmatrix} #1 & #2 & #3 \end{bmatrix}}$
    $\newcommand{\Meq}[3]{\begin{bmatrix} #1 \br #2 \br #3 \end{bmatrix}}$
    $\newcommand{\Mwe}[6]{\begin{bmatrix} #1 & #2 & #3\br #4 & #5 & #6 \end{bmatrix}}$
    $\newcommand{\Mew}[6]{\begin{bmatrix} #1 & #2 \br #3 & #4 \br #5 & #6 \end{bmatrix}}$
    $\newcommand{\Mee}[9]{\begin{bmatrix} #1 & #2 & #3 \br #4 & #5 & #6 \br #7 & #8 & #9 \end{bmatrix}}$
  {{< /raw >}}
</div>


{{% definition name="Moment generating function (MGF)" status="" %}}

Let $X$ be a random variable, we define the **moment generating function** (or **transform**) of $X$ to be the function $M\_X: \R \to \R $ such that

$$M\_X(t) = E\brac{ e^{Xt}}, t \in \R $$

**Discrete**:

$$M\_X(t) = \sum\_{x \in \R} e^{xt} p\_X(t)$$

**Continuous**:

$$M\_X(t) = \int\_{ \R } e^{xt} f\_X(x) \d x$$

{{% /definition %}}

{{% example name="" %}}

Let $X$ be a random variable with $\begin{align\*}
\frac{ 1 }{ 2 } & x = 2 \br
\frac{ 1 }{ 6 } & x = 3 \br
\frac{ 1 }{ 3 } & x = 5 \br
0 & \otherwise
\end{align\*}$

$M\_X(t) = E\brac{ e^{Xt}} = \frac{ 1 }{ 2 } e^{2t} + \frac{ 1 }{ 6 } e^{3t} + \frac{ 1 }{ 3 } e^{5t}$

{{% /example %}}

{{% lemma name="The MGF associated with a linear function of a Random Variable" index="" %}}

Let $M\_X(s)$ be the transform associated with a random variable $X$. Consider a new random variable $Y = aX + b$, $ a, b \in \R $.

$$M\_Y(t) = e^{bt} M\_X(at)$$

{{% proof index="" method="" %}}

$M\_Y(t) = E\brac{ e^{yt}} = E\brac{ e^{(aX + b)t}} = E\brac{ e^{(at)x} e^{bt}} = e^{bt} E\brac{ e^{(at)X}}$

{{% /proof %}}

{{% /lemma %}}

{{% example name="" %}}

$Y \text{~} N(\mu, \sigma^2), X \text{~} N(0, 1)$

$Y = \sigma X + \mu $

$f\_X(x) = \frac{ 1 }{ \sqrt[  ]{ 2 \pi }} e ^{- \frac{ x^2 }{ 2 }} $


$M\_X(t) = \int\_{ \R } e^{xt} f\_X(x) \d x = \int\_{ \R } \frac{ 1 }{ \sqrt[  ]{ 2 \pi } e ^{ - \frac{ x^2 }{ 2 }}} \d x = \int\_{ \R } e^{ - (\frac{ x^2 }{ 2 } - xt + \frac{ t^2 }{ 2 })} e^{ \frac{ t^2 }{ 2 }} \d x = e^ { \frac{ t^2 }{ 2 }}$

{{% /example %}}

{{% example name="" %}}

$X \text{~} \text{ Poisson}(\lambda) , p\_X(k) = \begin{cases}
  \frac{\lambda^k}{k!} e^{-\lambda} & k = 0, 1, 2, ... \br
  0 & \otherwise
\end{cases}$

$M\_X(t) = \sum\_{ k = 0 }^{ \infty } e^{kt} \frac{ \lambda^k e^{- \lambda}}{ k! } = e ^{ - \lambda } e^{ e^t \lambda } = e^{ \lambda (e^t - 1)}, \forall t \in \R$

{{% /example %}}

{{% remarks name="" %}}

$M\_X(t)$ may not be defined for all $t \in \R $

$f\_X(x) = \begin{cases}
  \frac{ 1 }{ x^2 } & x \geq 1\br
  0, & x < 1
\end{cases}$

$M\_X(t) = \int\_{ 1 }^{ \infty } \frac{ e^{xt}}{ x^2 } \d x $ does not converge for $t > 0 $

$\int\_{ \R } x \d x = \int\_{ 1 }^{ \infty } \frac{ 1 }{ x^2 } \d x = 1$

Moment generating function is only defined for $(-\infty, 0]$.

{{% /remarks %}}

{{% remarks name="" %}}

For $t = 0 $, $M\_X(0) = E\brac{ e^{0x}} = E\brac{ 1 } = 1$

If $h: \R \to \R $ such that $h(0) \neq 1 $, then $h $ cannot be the MGF function for some random variable $X$.

That is, here is no random variable $X$, such that $M\_X(t) = h(t), \forall t \in \R$.

{{% /remarks %}}


{{% theorem name="Inversion theorem" index="" status="" %}}

Let $X $ and $Y $ be two random variable with $M\_X(t) $ and $M\_Y(t) $ defined for all $t \in \R $  (for all $t$ in some open interval $(a, b)$ in $\R$). If $M\_X(t) = M\_Y(t), \forall t \in \R$($\forall t \in (a, b)$).

Then $F\_X(s) = F\_Y(s)  \forall s \in R$. $X $ and $Y $ have the same distribution.

{{% /theorem %}}

{{% example name="" %}}

Suppose a random variable $X $ has MGF given  as

$$M\_X(t) = \frac{ 1 }{ y } e^{-t} + \frac{ 1 }{ 2 } + \frac{ 1 }{ 8 } e^{yt} + \frac{ 1 }{ 8 } e^{5t} $$


What is the distribution of $X $

$$ p\_X(x) = \begin{cases}
  \frac{ 1 }{ 4 } &  x = -1 \br
  \frac{ 1 }{ 2 } & x= 0 \br
  \frac{ 1 }{ 8 } & x = 4 \br
  \frac{ 1 }{ 8 } & x = 5 \br
  0 & \otherwise
\end{cases} $$

{{% /example %}}

{{% note name="" %}}

Recall that the nth moment of a random variable $X $ is $E\brac{ X^n } $ from MGF to moments.

$\der{  }{ t } M\_X(t) = \der{  }{ t } E\brac{ e^{xt}} = E\brac{ \der{  }{ t } e^{xt}} = E\brac{ x e^{xt}} $

$\der{  }{ t } M\_X(t) \big |\_{t = 0} = E\brac{ X } $

$E\brac{  e^{xt}}  = E\brac{ 1 + \frac{ xt }{ 1 ! } + \frac{ \pare{xt}^2 }{ 2! } + ... } = \sum\_{ n = 0 }^{ \infty } E\brac{ \frac{(xt)^n }{ n! }} = \sum\_{ n = 0 }^{ \infty } \frac{ E\brac{ X } t^n }{ n! } $

This is the "exponential" quality function for the sequence $E\brac{ X^2 } \big |^ \infty \_{n = 0} $

$\frac{ \d ^n }{ \d t^n  } E\brac{ e^{xt}} \big |\_{t = 0} = \frac{ \d ^n }{ \d  t^n } \frac{ \pare{E\brac{ x^n } t^n }}{ n! } \big |\_ {t = 0} = E\brac{ X^n } $

{{% /note %}}

{{% theorem name="" index="" status="" %}}

If $M\_X(t) $ is defined in a neighborhood of $0$ then

$$\frac{ \d ^n }{ \d t^n  } M\_X(t) \big | \_{t = 0} = E\brac{ X^n }$$

{{% proof index="" method="" %}}

Discrete:

$\der{  }{ t } (M\_X(t)) = \der{  }{ t } (\sum\_{ x \in \R } e^{xt p\_X(x)}) = \sum\_{ x \in \R } \der{  }{ t } \pare{e^{xt} p\_X(x)} = \sum\_{ x \in \R } x e^{xt} p\_X(x) $

$\frac{ \d ^n }{ \d t^n  } M\_X(t) = \sum\_{ r \in \R } x^n e^{xt} p\_X(x) $

$\der{  }{ t } M\_X(t) \big | \_{t = 0} = \sum\_{ x \in \R } x p\_X(x) = E\brac{ X } $
{{% /proof %}}

{{% /theorem %}}

{{% example name="" %}}

$X \text{~}\text{ Exp}(\lambda), \lambda > 0$

$f\_X(x) = \begin{cases}
  \lambda e^{ - \lambda }x & x \geq 0 \br
  0 & \otherwise
\end{cases}$

$M\_X(x) = \int\_{ x \in \R } e^{xt} f\_X(x) \d x = \int\_{ 0 }^{ \infty } e^{xt} (\lambda e^{ - \lambda x }) \d x = \lambda \int\_{ 0 }^{ \infty } e^{x (t - \lambda)} \d x $

for $t < \lambda $

$= \frac{ \lambda }{ t - \lambda } e^{x (t - \lambda)} \big | ^ \infty \_0 = \frac{ \lambda^0 }{ t - \lambda } (0 - 1) = \frac{  \lambda }{  \lambda - t } $

$\der{  }{ t } M\_X(t) \big | \_{t = 0} = \frac{ \lambda }{(\lambda - t)^2  } \big | \_{t = 0} = \frac{ 1 }{ \lambda } = E\brac{ X } $

$\frac{ \d ^n }{ \d t^n }  M\_X(t) \big | \_{t = 0} = \frac{ n! }{ \lambda^n }$(by induction)

Note that $\frac{ \lambda }{ \lambda - t } = \frac{ 1 }{ 1 - \frac{ t }{ \lambda }} = 1 + \frac{  t }{ \lambda } + \frac{ t^2 }{  \lambda^2 } + ... = \sum\_{ n=0 }^{ \infty } \frac{ t^n }{ \lambda^n }$

{{% /example %}}

