---
title: "The set N of Natural Numbers"
date: 2018-08-06T11:03:48+08:00
volumes: ["1"]
layout: "note"
type: "notes"
issue: 1
weight: 11

---


<!--more-->

<div class="latex-macros">
  {{< raw >}}
    $\newcommand{\br}{\\}$

    $\newcommand{\R}{\mathbb{R}}$
    $\newcommand{\Q}{\mathbb{Q}}$
    $\newcommand{\Z}{\mathbb{Z}}$
    $\newcommand{\N}{\mathbb{N}}$
    $\newcommand{\C}{\mathbb{C}}$
    $\newcommand{\P}{\mathbb{P}}$
    $\newcommand{\F}{\mathbb{F}}$
    $\newcommand{\L}{\mathcal{L}}$
    $\newcommand{\spa}[1]{\text{span}(#1)}$
    $\newcommand{\set}[1]{\{#1\}}$
    $\newcommand{\emptyset}{\varnothing}$
    $\newcommand{\otherwise}{\text{ otherwise }}$
    $\newcommand{\if}{\text{ if }}$
    $\newcommand{\proj}{\text{proj}}$
    $\newcommand{\union}{\cup}$
    $\newcommand{\intercept}{\cap}$
    $\newcommand{\abs}[1]{| #1 |}$
    $\newcommand{\norm}[1]{\left\lVert#1\right\rVert}$
    $\newcommand{\pare}[1]{\left\(#1\right\)}$
    $\newcommand{\t}[1]{\text{ #1 }}$
    $\newcommand{\head}{\text H}$
    $\newcommand{\tail}{\text T}$
    $\newcommand{\d}{\text d}$
    $\newcommand{\limu}[2]{\underset{#1 \to #2}\lim}$
    $\newcommand{\inv}[1]{{#1}^{-1}}$
    $\newcommand{\inner}[2]{\langle #1, #2 \rangle}$
    $\newcommand{\nullity}[1]{\text{nullity}(#1)}$
    $\newcommand{\rank}[1]{\text{rank }#1}$
    $\newcommand{\var}[1]{\text{var}(#1)}$
    $\newcommand{\tr}[1]{\text{tr}(#1)}$
    $\newcommand{\oto}{\text{ one-to-one }}$
    $\newcommand{\ot}{\text{ onto }}$
    $\newcommand{\Re}[1]{\text{Re}(#1)}$
    $\newcommand{\Im}[1]{\text{Im}(#1)}$


    $\newcommand{\Vcw}[2]{\begin{bmatrix} #1 \br #2 \end{bmatrix}}$
    $\newcommand{\Vce}[3]{\begin{bmatrix} #1 \br #2 \br #3 \end{bmatrix}}$
    $\newcommand{\Vcr}[4]{\begin{bmatrix} #1 \br #2 \br #3 \br #4 \end{bmatrix}}$
    $\newcommand{\Vct}[5]{\begin{bmatrix} #1 \br #2 \br #3 \br #4 \br #5 \end{bmatrix}}$
    $\newcommand{\Vcy}[6]{\begin{bmatrix} #1 \br #2 \br #3 \br #4 \br #5 \br #6 \end{bmatrix}}$
    $\newcommand{\Vcu}[7]{\begin{bmatrix} #1 \br #2 \br #3 \br #4 \br #5 \br #6 \br #7 \end{bmatrix}}$

    $\newcommand{\vcw}[2]{\begin{matrix} #1 \br #2 \end{matrix}}$
    $\newcommand{\vce}[3]{\begin{matrix} #1 \br #2 \br #3 \end{matrix}}$
    $\newcommand{\vcr}[4]{\begin{matrix} #1 \br #2 \br #3 \br #4 \end{matrix}}$
    $\newcommand{\vct}[5]{\begin{matrix} #1 \br #2 \br #3 \br #4 \br #5 \end{matrix}}$
    $\newcommand{\vcy}[6]{\begin{matrix} #1 \br #2 \br #3 \br #4 \br #5 \br #6 \end{matrix}}$
    $\newcommand{\vcu}[7]{\begin{matrix} #1 \br #2 \br #3 \br #4 \br #5 \br #6 \br #7 \end{matrix}}$

    $\newcommand{\Mqw}[2]{\begin{bmatrix} #1 & #2 \end{bmatrix}}$
    $\newcommand{\Mqe}[3]{\begin{bmatrix} #1 & #2 & #3 \end{bmatrix}}$
    $\newcommand{\Mqr}[4]{\begin{bmatrix} #1 & #2 & #3 & #4 \end{bmatrix}}$
    $\newcommand{\Mqt}[5]{\begin{bmatrix} #1 & #2 & #3 & #4 & #5 \end{bmatrix}}$

    $\newcommand{\Mwq}[2]{\begin{bmatrix} #1 \br #2 \end{bmatrix}}$
    $\newcommand{\Meq}[3]{\begin{bmatrix} #1 \br #2 \br #3 \end{bmatrix}}$
    $\newcommand{\Mrq}[4]{\begin{bmatrix} #1 \br #2 \br #3 \br #4 \end{bmatrix}}$
    $\newcommand{\Mtq}[5]{\begin{bmatrix} #1 \br #2 \br #3 \br #4 \br #5 \end{bmatrix}}$

    $\newcommand{\Mqw}[2]{\begin{bmatrix} #1 & #2 \end{bmatrix}}$
    $\newcommand{\Mwq}[2]{\begin{bmatrix} #1 \br #2 \end{bmatrix}}$
    $\newcommand{\Mww}[4]{\begin{bmatrix} #1 & #2 \br #3 & #4 \end{bmatrix}}$
    $\newcommand{\Mqe}[3]{\begin{bmatrix} #1 & #2 & #3 \end{bmatrix}}$
    $\newcommand{\Meq}[3]{\begin{bmatrix} #1 \br #2 \br #3 \end{bmatrix}}$
    $\newcommand{\Mwe}[6]{\begin{bmatrix} #1 & #2 & #3\br #4 & #5 & #6 \end{bmatrix}}$
    $\newcommand{\Mew}[6]{\begin{bmatrix} #1 & #2 \br #3 & #4 \br #5 & #6 \end{bmatrix}}$
    $\newcommand{\Mee}[9]{\begin{bmatrix} #1 & #2 & #3 \br #4 & #5 & #6 \br #7 & #8 & #9 \end{bmatrix}}$
  {{< /raw >}}
</div>

{{% definition name="Natural Numbers $\N$" status="" %}}

The set of all positive integers ${1, 2, 3, ...}$ are natural numbers, denoted by $\N$.

{{% /definition %}}

{{% axioms name="Peano Axioms (Peano Postulates)" status="warning" %}}

**N1.** $1$ belongs to $\N $.

**N2.** If $n$ belongs to $\N$ then its successor $n + 1$ belongs to $\N$.

**N3.** $1$ is not the successor of any element in $\N$.

**N4.** If $n$ and $m$ in $\N$ have the same successor, then $n = m$.

**N5. (Principal of Induction)** A subset of $\N $ which contains $1$, and which contains $n + 1$ whenever it contains $n $, must equal $\N $.

{{% /axioms %}}

{{% definition name="proposition" status="" %}}

A **proposition** is a mathematical statement, usually denoted by $P$.

$P(n) $ is a proposition about $n$.

{{% /definition %}}

{{% theorem name="Well-ordering Principle of Natural Numbers" index="" status="warning" %}}

**N5'.** Every nonempty subset of $\N$ has a minimal element.

{{% proof index="" method="strong induction" %}}

Let $A$ be a non-empty subset of $\N $. Want to know that $A $ has a minimal element, that is, there is an element $a \in A $ such that $a \leq n $ for all $n \in A $. We will do this by strong induction on the following predicate:

$$P(n): \text{If }n \in A\text{, then }A\text{ has a minimal element.} $$

**the base case:** $P(0)$ is clearly true, since $0 \leq n \forall n \in N $.

**the inductive step:** Want to show that $[P(0) \land P(1) \land P(2) \land ... \land P(n)] \to P(n + 1)$.

To this end, suppose that $P(0), P(1), ..., P(n) $ are all true and that $n + 1 \in A$. We consider two cases.

*CASE 1*: $\neg \exists m (m \in A \land m < n + 1) $

In this case,  $n + 1$ is the least element of $A$.

*CASE 2*: $\exists m (m \in A \land m < n + 1) $

In this case, since $P(m)$ is true, $A$ has a least element.

Either way, we conclude that $P(n + 1)$ is true.

So, by strong mathematical induction, we obtain that $P(n) $ is true for all $n \in N$. Since $A $ is not empty, we can pick an $n \in A $. Moreover, since $P(n) $ is true, this implies that $A $ has a least element.

{{% /proof %}}

**N1** - **N4**, **N5** $\iff$ **N1** - **N4**, **N5'**

{{% /theorem %}}

{{% corollary name="" index="" %}}

**O1.** For $a,b \in \N, a \leq b $ or $b \leq a $.

**O2.** $a \leq b, b \leq a \implies a = b $.

**O3.** $a \leq b, b \leq c \implies a \leq c $.

{{% /corollary %}}

{{% example name="" status="warning" %}}

Prove that **N1** - **N4**, **N5** $\implies$  $\forall x \in X, x \neq 1$ is a successor in $X $.

{{% proof index="" name="" %}}

Let $X$ be a subset of $\N$,

Assume that $x \neq 1$ and $x$ not a successor.

Let $X$ be a set of $\set{ 1 } \cup \set{ \text{all successors}} = \N$ by **N5**.

Then $x \in X , x \neq 1$ is CONTRADICTION; $x$ is a successor.

{{% /proof %}}

{{% /example %}}

{{% definition name="Mathematical induction" status="" %}}

**Mathematical induction** is a mathematical proof technique used to prove that a property $P(n)$ holds for every natural number $n$.

The proof consists of <u>two steps</u>:

1. The **base case**: prov that the statement holds for the first natural number $n\_1 $.
2. The **inductive step**: assume the statement holds for some natural number $n $, and prove that then the statement holds for $n + 1 $.

The hypothesis in the inductive step, that the statement holds for some $n$, is called the **induction hypothesis** or **inductive hypothesis**.

{{% /definition %}}

{{% example name="Mathematical induction" index="1" %}}

$P(n) = 1 + 3 + 5 + ... + 2n - 1 =  n^2$

$P(1) = 1 = 1^2$

$P(2) = 1 + 3 = 4 = 2^2 $

Assume $P(n)$:

Then $1 + 3 + 5 + ... + 2n -1  = n^2 $

$1 + 3 + 5 + ... + 2n + 1 = n^2 + 2n + 1 $

$1 + 3 + 5 + ... + (2(n+1) - 1) = (n+1)^2 $

So $\P(n) \implies \P(n+1) $.

{{% /example %}}

{{% definition name="Complete Induction (Strong Induction)" status="" %}}

**Complete induction** is a variant of mathematical induction which has a stronger inductive hypothesis. The hypothesis assumes that $P(n) $ holds for **all** natural $n $ less than or equals to $n$.

The proof still consists of <u>two steps</u>:

1. The **base case**: prov that the statement holds for the first natural number $n\_1 $.
2. The **inductive step**: assume the statement holds for all natural numbers $\leq n$, and prove that then the statement holds for $n + 1 $.

{{% /definition %}}

{{% example name="" %}}

Try to prove that $N1 - N4, N5 \iff N1, ..., N4, N5' $

{{% /example %}}

{{% example name="Prime factorization" %}}

Every $n \in \N$ is a product of primes.

Let $P(n)$: $n$ is a product of primes.

Assume $P(m)$ is product of primes for all $m \leq n $.

For $n + 1$,

if $n+1$ prime, then $n + 1$ is a product of prime.

if $n+1$ not prime (composite), then $n + 1 = a \cdot b$ for some $a, b  \in \N$, $a,b  > 1$.

$\therefore$ by complete induction

$$a = p\_1, p\_2, ..., p\_{ k } $$

$$b = q\_1, q\_2, ..., q\_{ l } $$

$\therefore n + 1 = ab = p\_1 p\_2 ... p\_{ k } q\_1 q\_2 ... q\_{ l } $

$\therefore P(n + 1)$

Note: For $P(1)$, allow $1 $ to be a prime.

{{% /example %}}

{{% example name="" %}}

$P(n): \abs{ \sin(nx)} \leq n \abs{ \sin(x)} $

If $n = 1$, $\abs{ \sin (1 x)} \leq 1 \abs{ \sin x }$

Assume $P(n)$ consider

$\abs{ \sin ((n + 1) x)} = \abs{ \sin nx \cos x + \cos nx \sin x}$

$\abs{ a + b } \leq \abs{ a } + \abs{ b }$(triangle inequality)

$\therefore $

$\begin{align\*}
\abs{ \sin((n+1)x)} &\leq \abs{ \sin nx \cos x } + \abs{ \cos nx \sin x } \br
& \leq \abs{ \sin nx } \abs{ \cos x } + \abs{ \cos nx } \abs{ \sin x } \br
& \leq \abs{ \sin nx } \cdot 1 + 1 \cdot \abs{ \sin x } \br
& \leq n \abs{ \sin x } + \abs{  \sin x } = (n+1) \abs{ \sin x }
\end{align\*}$

$\therefore P(n + 1)$.

{{% /example %}}


