---
title: "The exponential and logarithm functions"
date: 2019-03-13T16:39:00+08:00
volumes: ["11"]
layout: "note"
type: "notes"
issue: 5
weight: 115

---

<!--more-->

<div class="latex-macros">
  {{< raw >}}
    $\newcommand{\br}{\\}$
    $\newcommand{\R}{\mathbb{R}}$
    $\newcommand{\Q}{\mathbb{Q}}$
    $\newcommand{\Z}{\mathbb{Z}}$
    $\newcommand{\N}{\mathbb{N}}$
    $\newcommand{\C}{\mathbb{C}}$
    $\newcommand{\P}{\mathbb{P}}$
    $\newcommand{\F}{\mathbb{F}}$
    $\newcommand{\L}{\mathcal{L}}$
    $\newcommand{\spa}[1]{\text{span}(#1)}$
    $\newcommand{\dist}[1]{\text{dist}(#1)}$
    $\newcommand{\max}[1]{\text{max}(#1)}$
    $\newcommand{\min}[1]{\text{min}(#1)}$
    $\newcommand{\supr}{\text{sup}}$
    $\newcommand{\infi}{\text{inf}}$
    $\newcommand{\ite}[1]{\text{int}(#1)}$
    $\newcommand{\ext}[1]{\text{ext}(#1)}$
    $\newcommand{\bdry}[1]{\partial #1}$
    $\newcommand{\argmax}[1]{\underset{#1}{\text{argmax }}}$
    $\newcommand{\argmin}[1]{\underset{#1}{\text{argmin }}}$
    $\newcommand{\set}[1]{\left\{#1\right\}}$
    $\newcommand{\emptyset}{\varnothing}$
    $\newcommand{\tilde}{\text{~}}$
    $\newcommand{\otherwise}{\text{ otherwise }}$
    $\newcommand{\if}{\text{ if }}$
    $\newcommand{\proj}{\text{proj}}$
    $\newcommand{\union}{\cup}$
    $\newcommand{\intercept}{\cap}$
    $\newcommand{\abs}[1]{\left| #1 \right|}$
    $\newcommand{\norm}[1]{\left\lVert#1\right\rVert}$
    $\newcommand{\pare}[1]{\left(#1\right)}$
    $\newcommand{\brac}[1]{\left[#1\right]}$
    $\newcommand{\t}[1]{\text{ #1 }}$
    $\newcommand{\head}{\text H}$
    $\newcommand{\tail}{\text T}$
    $\newcommand{\d}{\text d}$
    $\newcommand{\limu}[2]{\underset{#1 \to #2}\lim}$
    $\newcommand{\limsupu}[2]{\underset{#1 \to #2}{\lim\supr}}$
    $\newcommand{\liminfu}[2]{\underset{#1 \to #2}{\lim\infi}}$
    $\newcommand{\limd}[3]{\underset{#1 \to #2; #3}\lim}$
    $\newcommand{\der}[2]{\frac{\d #1}{\d #2}}$
    $\newcommand{\derw}[2]{\frac{\d #1^2}{\d^2 #2}}$
    $\newcommand{\pder}[2]{\frac{\partial #1}{\partial #2}}$
    $\newcommand{\pderw}[2]{\frac{\partial^2 #1}{\partial #2^2}}$
    $\newcommand{\pderws}[3]{\frac{\partial^2 #1}{\partial #2 \partial #3}}$
    $\newcommand{\inv}[1]{{#1}^{-1}}$
    $\newcommand{\inner}[2]{\langle #1, #2 \rangle}$
    $\newcommand{\nullity}[1]{\text{nullity}(#1)}$
    $\newcommand{\rank}[1]{\text{rank }#1}$
    $\newcommand{\nullspace}[1]{\mathcal{N}\pare{#1}}$
    $\newcommand{\range}[1]{\mathcal{R}\pare{#1}}$
    $\newcommand{\var}[1]{\text{var}\pare{#1}}$
    $\newcommand{\cov}[2]{\text{cov}(#1, #2)}$
    $\newcommand{\tr}[1]{\text{tr}(#1)}$
    $\newcommand{\oto}{\text{ one-to-one }}$
    $\newcommand{\ot}{\text{ onto }}$
    $\newcommand{\ipto}{\overset{\text{i.p.}}\longrightarrow}$
    $\newcommand{\asto}{\overset{\text{a.s.}}\longrightarrow}$
    $\newcommand{\expdist}[1]{\text{ ~ Exp}(#1)}$
    $\newcommand{\unifdist}[1]{\text{ ~ Unif}(#1)}$
    $\newcommand{\normdist}[2]{\text{ ~ N}(#1,#2)}$
    $\newcommand{\berndist}[2]{\text{ ~ Bernoulli}(#1,#2)}$
    $\newcommand{\geodist}[1]{\text{ ~ Geometric}(#1)}$
    $\newcommand{\poissondist}[1]{\text{ ~ Poisson}(#1)}$
    $\newcommand{\ceil}[1]{\lceil#1\rceil}$
    $\newcommand{\floor}[1]{\lfloor#1\rfloor}$
    $\newcommand{\Re}[1]{\text{Re}(#1)}$
    $\newcommand{\Im}[1]{\text{Im}(#1)}$
    $\newcommand{\dom}[1]{\text{dom}(#1)}$
    $\newcommand{\fnext}[1]{\overset{\sim}{#1}}$
    $\newcommand{\transpose}[1]{{#1}^{\text{T}}}$
    $\newcommand{\b}[1]{\boldsymbol{#1}}$
    $\newcommand{\None}[1]{}$
    $\newcommand{\Vcw}[2]{\begin{bmatrix} #1 \br #2 \end{bmatrix}}$
    $\newcommand{\Vce}[3]{\begin{bmatrix} #1 \br #2 \br #3 \end{bmatrix}}$
    $\newcommand{\Vcr}[4]{\begin{bmatrix} #1 \br #2 \br #3 \br #4 \end{bmatrix}}$
    $\newcommand{\Vct}[5]{\begin{bmatrix} #1 \br #2 \br #3 \br #4 \br #5 \end{bmatrix}}$
    $\newcommand{\Vcy}[6]{\begin{bmatrix} #1 \br #2 \br #3 \br #4 \br #5 \br #6 \end{bmatrix}}$
    $\newcommand{\Vcu}[7]{\begin{bmatrix} #1 \br #2 \br #3 \br #4 \br #5 \br #6 \br #7 \end{bmatrix}}$
    $\newcommand{\vcw}[2]{\begin{matrix} #1 \br #2 \end{matrix}}$
    $\newcommand{\vce}[3]{\begin{matrix} #1 \br #2 \br #3 \end{matrix}}$
    $\newcommand{\vcr}[4]{\begin{matrix} #1 \br #2 \br #3 \br #4 \end{matrix}}$
    $\newcommand{\vct}[5]{\begin{matrix} #1 \br #2 \br #3 \br #4 \br #5 \end{matrix}}$
    $\newcommand{\vcy}[6]{\begin{matrix} #1 \br #2 \br #3 \br #4 \br #5 \br #6 \end{matrix}}$
    $\newcommand{\vcu}[7]{\begin{matrix} #1 \br #2 \br #3 \br #4 \br #5 \br #6 \br #7 \end{matrix}}$
    $\newcommand{\Mqw}[2]{\begin{bmatrix} #1 & #2 \end{bmatrix}}$
    $\newcommand{\Mqe}[3]{\begin{bmatrix} #1 & #2 & #3 \end{bmatrix}}$
    $\newcommand{\Mqr}[4]{\begin{bmatrix} #1 & #2 & #3 & #4 \end{bmatrix}}$
    $\newcommand{\Mqt}[5]{\begin{bmatrix} #1 & #2 & #3 & #4 & #5 \end{bmatrix}}$
    $\newcommand{\Mwq}[2]{\begin{bmatrix} #1 \br #2 \end{bmatrix}}$
    $\newcommand{\Meq}[3]{\begin{bmatrix} #1 \br #2 \br #3 \end{bmatrix}}$
    $\newcommand{\Mrq}[4]{\begin{bmatrix} #1 \br #2 \br #3 \br #4 \end{bmatrix}}$
    $\newcommand{\Mtq}[5]{\begin{bmatrix} #1 \br #2 \br #3 \br #4 \br #5 \end{bmatrix}}$
    $\newcommand{\Mqw}[2]{\begin{bmatrix} #1 & #2 \end{bmatrix}}$
    $\newcommand{\Mwq}[2]{\begin{bmatrix} #1 \br #2 \end{bmatrix}}$
    $\newcommand{\Mww}[4]{\begin{bmatrix} #1 & #2 \br #3 & #4 \end{bmatrix}}$
    $\newcommand{\Mqe}[3]{\begin{bmatrix} #1 & #2 & #3 \end{bmatrix}}$
    $\newcommand{\Meq}[3]{\begin{bmatrix} #1 \br #2 \br #3 \end{bmatrix}}$
    $\newcommand{\Mwe}[6]{\begin{bmatrix} #1 & #2 & #3\br #4 & #5 & #6 \end{bmatrix}}$
    $\newcommand{\Mew}[6]{\begin{bmatrix} #1 & #2 \br #3 & #4 \br #5 & #6 \end{bmatrix}}$
    $\newcommand{\Mee}[9]{\begin{bmatrix} #1 & #2 & #3 \br #4 & #5 & #6 \br #7 & #8 & #9 \end{bmatrix}}$
  {{< /raw >}}
</div>

{{% definition name="Exponential function" status="" %}}

$\forall x \in \R $, we define the **exponential function** $\exp(x) $ to be the real number 

$$\exp(x) = \sum\_{ n=0 }^{ \infty } \frac{ x^n }{ n! } $$

{{% /definition %}}

{{% theorem name="Basic properties of exponential" index="" status="" %}}

1. $\forall x \in \R, \sum\_{ n=0 }^{ \infty } \frac{ x^n }{ n! } $ is absolutely
convergent. <br>
In particular, $\forall x \in \R, \exp (x), \exists \exp(x) \in \R $. <br>
$\sum\_{ n=0 }^{ \infty } \frac{ x^n }{ n! } $ has an infinite radius of convergence, and $\exp $ is a real analytic function on $(- \infty, \infty)$.
2. $\exp$ is **differentiable** on $\R $, and for every $x \in \R $, $\exp'(x) = \exp (x) $.
3. $\exp$ is **continuous** on $\R $, and for every interval $[a,b] $, we have 
$\int\_{ [a,b] } \exp (x) \d x = \exp (b) - \exp (a)$
4. $\forall x, y \in \R, \exp (x + y) = \exp (x) \exp (y). $
5. $\exp (0) = 1. \forall x \in \R, \exp (x) > 0, \exp (-x) = \frac{ 1 }{ \exp (x)}$
6. $\exp$ is strictly monotone increasing.

{{% /theorem %}}

{{% definition name="Euler's Number" status="" %}}

The number $e$ is defined to be

$$e \triangleq \exp (1) = \sum\_{ n=0 }^{ \infty } = \frac{ 1 }{ 0! } + \frac{ 1 }{ 1! } + \frac{ 1 }{ 2! } + \frac{ 1 }{ 3! } + ... $$

{{% /definition %}}

{{% proposition name="" index="" status="" %}}

$$\forall x \in \R, \exp (x) = e^x$$

{{% /proposition %}}

{{% definition name="Logorithm" status="" %}}

We define the **natural logarithm function** $\ln : (0, \infty) \to \R$ to be the
inverse of the exponential function. Thus $\exp \ln x = x $ and $\ln  \exp  x = x $.

{{% /definition %}}

{{% theorem name="Logarithm properties" index="" status="" %}}

1. $\forall x \in (0, \infty), \ln ' (x) = \frac{ 1 }{ x } $. <br>
In particular, by the fundamental theorem of calculus, we have $\int\_{ [a, b] } \frac{ 1 }{ x } \d x = \ln (b) - \ln (a)$ for any interval $[a, b] \subseteq (0, \infty)$
2. $\forall x, y \in (0, \infty), \ln (xy) = \ln (x) + \ln (y)$.
3. $\forall x \in (i, \infty), \ln (1) = 0, \ln (\frac{ 1 }{ x }) = - \ln (x).$
4. $\forall x \in (0, \infty) , y \in \R, \ln (x^y) = y \ln (x).$
5. $\forall x \in (-1, 1), \ln (1-x) = - \sum\_{ n=1 }^{ \infty } \frac{ x^n }{ n }.$<br>
In particular, $\ln$ is analytic at $1$, with the power series expansion
$$\ln (x) = \sum\_{ n=1 }^{ \infty } \frac{(-1)^{n+1}}{ n } (x-1)^n $$

for $x \in (0,2) $, with radius of convergence $1$.

{{% /theorem %}}

{{% example name="Application of Abel's theorem" %}}

TODO:

{{% /example %}}
