---
title: "Alternating Series and Integral Tests"
date: 2018-08-22T11:00:48+08:00
volumes: ["2"]
layout: "note"
issue: 9
weight: 29

---

<!--more-->

<div class="latex-macros">
  {{< raw >}}
    $\newcommand{\br}{\\}$

    $\newcommand{\R}{\mathbb{R}}$
    $\newcommand{\Q}{\mathbb{Q}}$
    $\newcommand{\Z}{\mathbb{Z}}$
    $\newcommand{\N}{\mathbb{N}}$
    $\newcommand{\C}{\mathbb{C}}$
    $\newcommand{\P}{\mathbb{P}}$
    $\newcommand{\F}{\mathbb{F}}$
    $\newcommand{\L}{\mathcal{L}}$
    $\newcommand{\spa}[1]{\text{span}(#1)}$
    $\newcommand{\dist}[1]{\text{dist}(#1)}$
    $\newcommand{\max}[1]{\text{max}(#1)}$
    $\newcommand{\min}[1]{\text{min}(#1)}$
    $\newcommand{\supr}[1]{\text{sup}(#1)}$
    $\newcommand{\infi}[1]{\text{inf}(#1)}$
    $\newcommand{\set}[1]{\{#1\}}$
    $\newcommand{\emptyset}{\varnothing}$
    $\newcommand{\otherwise}{\text{ otherwise }}$
    $\newcommand{\if}{\text{ if }}$
    $\newcommand{\proj}{\text{proj}}$
    $\newcommand{\union}{\cup}$
    $\newcommand{\intercept}{\cap}$
    $\newcommand{\abs}[1]{| #1 |}$
    $\newcommand{\norm}[1]{\left\lVert#1\right\rVert}$
    $\newcommand{\pare}[1]{\left(#1\right)}$
    $\newcommand{\t}[1]{\text{ #1 }}$
    $\newcommand{\head}{\text H}$
    $\newcommand{\tail}{\text T}$
    $\newcommand{\d}{\text d}$
    $\newcommand{\limu}[2]{\underset{#1 \to #2}\lim}$
    $\newcommand{\inv}[1]{{#1}^{-1}}$
    $\newcommand{\inner}[2]{\langle #1, #2 \rangle}$
    $\newcommand{\nullity}[1]{\text{nullity}(#1)}$
    $\newcommand{\rank}[1]{\text{rank }#1}$
    $\newcommand{\var}[1]{\text{var}(#1)}$
    $\newcommand{\tr}[1]{\text{tr}(#1)}$
    $\newcommand{\oto}{\text{ one-to-one }}$
    $\newcommand{\ot}{\text{ onto }}$
    $\newcommand{\Re}[1]{\text{Re}(#1)}$
    $\newcommand{\Im}[1]{\text{Im}(#1)}$


    $\newcommand{\Vcw}[2]{\begin{bmatrix} #1 \br #2 \end{bmatrix}}$
    $\newcommand{\Vce}[3]{\begin{bmatrix} #1 \br #2 \br #3 \end{bmatrix}}$
    $\newcommand{\Vcr}[4]{\begin{bmatrix} #1 \br #2 \br #3 \br #4 \end{bmatrix}}$
    $\newcommand{\Vct}[5]{\begin{bmatrix} #1 \br #2 \br #3 \br #4 \br #5 \end{bmatrix}}$
    $\newcommand{\Vcy}[6]{\begin{bmatrix} #1 \br #2 \br #3 \br #4 \br #5 \br #6 \end{bmatrix}}$
    $\newcommand{\Vcu}[7]{\begin{bmatrix} #1 \br #2 \br #3 \br #4 \br #5 \br #6 \br #7 \end{bmatrix}}$

    $\newcommand{\vcw}[2]{\begin{matrix} #1 \br #2 \end{matrix}}$
    $\newcommand{\vce}[3]{\begin{matrix} #1 \br #2 \br #3 \end{matrix}}$
    $\newcommand{\vcr}[4]{\begin{matrix} #1 \br #2 \br #3 \br #4 \end{matrix}}$
    $\newcommand{\vct}[5]{\begin{matrix} #1 \br #2 \br #3 \br #4 \br #5 \end{matrix}}$
    $\newcommand{\vcy}[6]{\begin{matrix} #1 \br #2 \br #3 \br #4 \br #5 \br #6 \end{matrix}}$
    $\newcommand{\vcu}[7]{\begin{matrix} #1 \br #2 \br #3 \br #4 \br #5 \br #6 \br #7 \end{matrix}}$

    $\newcommand{\Mqw}[2]{\begin{bmatrix} #1 & #2 \end{bmatrix}}$
    $\newcommand{\Mqe}[3]{\begin{bmatrix} #1 & #2 & #3 \end{bmatrix}}$
    $\newcommand{\Mqr}[4]{\begin{bmatrix} #1 & #2 & #3 & #4 \end{bmatrix}}$
    $\newcommand{\Mqt}[5]{\begin{bmatrix} #1 & #2 & #3 & #4 & #5 \end{bmatrix}}$

    $\newcommand{\Mwq}[2]{\begin{bmatrix} #1 \br #2 \end{bmatrix}}$
    $\newcommand{\Meq}[3]{\begin{bmatrix} #1 \br #2 \br #3 \end{bmatrix}}$
    $\newcommand{\Mrq}[4]{\begin{bmatrix} #1 \br #2 \br #3 \br #4 \end{bmatrix}}$
    $\newcommand{\Mtq}[5]{\begin{bmatrix} #1 \br #2 \br #3 \br #4 \br #5 \end{bmatrix}}$

    $\newcommand{\Mqw}[2]{\begin{bmatrix} #1 & #2 \end{bmatrix}}$
    $\newcommand{\Mwq}[2]{\begin{bmatrix} #1 \br #2 \end{bmatrix}}$
    $\newcommand{\Mww}[4]{\begin{bmatrix} #1 & #2 \br #3 & #4 \end{bmatrix}}$
    $\newcommand{\Mqe}[3]{\begin{bmatrix} #1 & #2 & #3 \end{bmatrix}}$
    $\newcommand{\Meq}[3]{\begin{bmatrix} #1 \br #2 \br #3 \end{bmatrix}}$
    $\newcommand{\Mwe}[6]{\begin{bmatrix} #1 & #2 & #3\br #4 & #5 & #6 \end{bmatrix}}$
    $\newcommand{\Mew}[6]{\begin{bmatrix} #1 & #2 \br #3 & #4 \br #5 & #6 \end{bmatrix}}$
    $\newcommand{\Mee}[9]{\begin{bmatrix} #1 & #2 & #3 \br #4 & #5 & #6 \br #7 & #8 & #9 \end{bmatrix}}$
  {{< /raw >}}
</div>

{{% example name="" %}}

We show $\sum\ \frac{ 1 }{ n } = +\infty$.



{{% proof index="" method="" %}}

$\sum\ \frac{ 1 }{ n } \geq \int\_{ 1 }^{ n+1 } \frac{ 1 }{ x } \d x = \log\_e(n+1)$

Since $\limu{ n }{ \infty } \log\_e(n+1) = + \infty , \sum\ \frac{ 1 }{ n } = + \infty$.

{{% note name="" %}}

We use integral test in this case. Notice how we choose the lower limit. It's pretty arbitrary as long as it is larger than $1$ and meet our need. Think about it, why can we do this.

{{% /note %}}

{{% /proof %}}

{{% /example %}}

{{% example name="" %}}

We show $\sum \frac{ 1 }{ n^2 }$ converges.

{{% proof index="" method="" %}}

$\sum\_{ k=1 }^{ n } \frac{ 1 }{ k^2 } \leq 1 + \int\_{ 1 }^{ n } \frac{ 1 }{ x^2 } \d x = 2 - \frac{ 1 }{ n } < 2$.

$\therefore \sum \frac{ 1 }{ n^2 }$ converges.

{{% /proof %}}

{{% /example %}}

{{% definition name="Alternating Series" status="" %}}

Let $a\_n >0 $, $\sum\_{ n = 1 }^{ \infty } (-1)^{n+1} a\_n$ is alternating.

any convergent series has $a\_n \to 0 $.

Suppose $a\_n > 0 $ and $a\_n \to 0 $

suppose $a\_n > a\_{n+1} \forall n$ i.e. decreasing.

{{% /definition %}}

{{% theorem name="" index="" status="" %}}

$\sum \frac{ 1 }{ n^p } $ converges if and only if $p > 1 $.

{{% /theorem %}}

{{% definition name="Alternating Series" status="" %}}

$\sum (-1)^{n+1} a\_n $ is called an alternating series.

{{% /definition %}}


{{% theorem name="Alternating Series Theorem" index="" status="" %}}

If $a\_1 \geq a\_2 \geq ... \geq a\_n \geq ... \geq 0 $ and $\lim a\_n = 0 $, then the alternating series $\sum\ (-1)^{n +1} a\_n $ converges. Moreover, the partial sums $s\_n = \sum\_{ k=1 }^{ n } (-1)^{k+1} a\_k $ satisfy $\abs{ s - s\_n } \leq a\_n $for all $n $.

{{% proof index="" method="" %}}

We need to show that the sequence $(s\_n)$ converges. Note that the subsequence $(s\_{2n}) $ is increasing because $s\_{2n+2} - s\_{2n} = + a\_{2n+1} - a\_{ 2n + 2 } \geq 0 $. Similarly, the subsequence $(s\_{2n-1}) $ is decreasing since $s\_{2n+1} - s\_{2n-1} = a\_{2n+1} - a\_{2n} \leq 0 $. We claim

$$s\_{2m} \leq s\_{2n+1} \forall m, n \in \N  \tag{1}$$

First note that $s\_{2n} \leq s\_{2n+1} $ for all $n $, because $s\_{2n+1} -s\_{2n} = a\_{2n+1} \geq 0$. If $m \leq n $, then $(1)$ holds because $s\_{2n+1} \geq s\_{2m+1} \geq s\_{2m} $. Thanks to $(1) $, we see that $(s\_{2n}) $ is an increasing subsequence of $(s\_n) $ bounded above by each odd partial sum, and $(s\_{2n+1}) $ is a decreasing subsequence of $(s\_n) $ bounded below by each even partial sum. By theorem 10.2, these subsequences converge, say to $s $ and $t $. Now

$$t - s = \limu{ n  }\infty{ s\_{2n+1}} - \limu{ n} \infty { s\_{2n}} = \limu{ n} \infty {(s\_{2n+1} - s\_{2n})} = \limu{ n} \infty { a\_{2n+1}} = 0 $$

so $s = t$. It follows that $\lim\_n s\_n = s$.

{{% /proof %}}

{{% /theorem %}}


